proof/refine/ARM/Ipc_R.thy
@@ -2976,18 +2976,22 @@ lemma schedContextResume_corres:
      apply wp
     apply wp
    apply (subgoal_tac "sc_tcb_sc_at (\<lambda>t. bound_sc_tcb_at (\<lambda>sc. sc = Some ptr) (the t) s) ptr s ")
-    apply (clarsimp simp: sc_at_ppred_def obj_at_def is_sc_obj_def bound_sc_tcb_at_def is_tcb_def)
+    apply (clarsimp simp: sc_at_ppred_def obj_at_def is_sc_obj_def bound_sc_tcb_at_def is_tcb_def
+                    cong: conj_cong)
     apply (intro conjI impI; (clarsimp simp: invs_def valid_state_def; fail)?)
-          apply (fastforce simp: invs_def valid_state_def valid_pspace_def valid_obj_def)
-         apply (clarsimp simp: is_schedulable_bool_def get_tcb_def obj_at_kh_kheap_simps)
-         apply (fastforce dest!: active_sc_valid_refillsE
-                           simp: valid_refills_def vs_all_heap_simps rr_valid_refills_def
-                          split: if_splits)
-        apply (fastforce simp: is_schedulable_bool_def get_tcb_def is_sc_active_def
-                               vs_all_heap_simps)
+           apply (fastforce simp: invs_def valid_state_def valid_pspace_def valid_obj_def)
+          apply (clarsimp simp: is_schedulable_bool_def get_tcb_def obj_at_kh_kheap_simps)
+          apply (fastforce simp: valid_refills_def vs_all_heap_simps rr_valid_refills_def
+                                 opt_map_left_Some MIN_REFILLS_def
+                          dest!: active_sc_valid_refillsE split: if_split_asm)
+         apply (clarsimp simp: is_schedulable_bool_def get_tcb_def is_sc_active_kh_simp)
+         apply (fastforce simp: valid_refills_def vs_all_heap_simps rr_valid_refills_def
+                          dest: active_sc_valid_refillsE)
+        apply (clarsimp simp: is_schedulable_bool_def get_tcb_def is_sc_active_def active_sc_def
+                               vs_all_heap_simps opt_map_left_Some)
        apply (prop_tac "is_active_sc ptr s")
         apply (fastforce simp: vs_all_heap_simps is_schedulable_bool_def get_tcb_def
-                               is_sc_active_def)
+                               is_sc_active_def opt_map_left_Some)
        apply (fastforce simp: vs_all_heap_simps valid_ready_qs_2_def
                               valid_ready_queued_thread_2_def in_ready_q_def)+
      apply (clarsimp simp: is_schedulable_bool_def get_tcb_def)
@@ -2997,16 +3001,23 @@ lemma schedContextResume_corres:
    apply (drule sym_refs_ko_atD[rotated], simp add: obj_at_def)
    apply (clarsimp simp: pred_tcb_at_def obj_at_def refs_of_rev)
   apply (clarsimp simp: invs'_def valid_state'_def valid_pspace'_def)
-  apply (intro conjI impI allI)
-    apply (fastforce simp: sc_at_ppred_def obj_at_def is_sc_obj_def valid_obj_def
-                     dest: invs_valid_objs intro!: sc_at_cross)
-   apply clarsimp
-  apply (clarsimp simp: state_relation_def obj_at_def sc_at_ppred_def)
-  apply (drule (1) pspace_relation_absD)
-  apply (clarsimp split: if_splits)
-  apply (clarsimp simp: sc_relation_def split: kernel_object.splits)
-  apply (simp only: sc_relation_def eq_commute[where a="Some P" for P])
-  apply (clarsimp simp: obj_at'_def projectKO_eq projectKO_sc)
+  apply (rule context_conjI; clarsimp?)
+   apply (fastforce simp: sc_tcb_sc_at_def obj_at_def is_sc_obj_def valid_obj_def
+                    dest: invs_valid_objs intro!: sc_at_cross)
+  apply (rule conjI, erule valid_objs'_valid_tcbs')
+  apply (clarsimp simp: sc_tcb_sc_at_def obj_at_def)
+  apply (frule (2) sym_ref_sc_tcb[OF invs_sym_refs], clarsimp)
+  apply (prop_tac "scTCB ko = Some y")
+   apply (frule state_relation_sc_relation[where ptr=ptr]; clarsimp simp: obj_at_simps is_sc_obj)
+     apply (erule (1) valid_sched_context_size_objsI[OF invs_valid_objs], simp)
+   apply (clarsimp simp: sc_relation_def projection_rewrites)
+  apply (frule_tac x=y in pspace_relation_absD[OF _ state_relation_pspace_relation]; simp)
+  apply (clarsimp simp: obj_at'_def projectKOs isSchedulable_bool_def projection_rewrites
+                        other_obj_relation_def tcb_relation_def)
+  apply (drule sym[where s="Some ptr"])
+  apply (clarsimp simp: projection_rewrites isScActive_def)
+  apply (erule (1) valid_objsE')
+  apply (clarsimp simp: valid_obj'_def valid_sched_context'_def sc_relation_def projection_rewrites)
   done
 
 lemma getScTime_wp:
