proof/refine/ARM/SchedContextInv_R.thy
@@ -384,15 +384,214 @@ lemma valid_sc_size_sc_relation:
   "\<lbrakk>valid_sched_context_size n; sc_relation sc n sc'\<rbrakk> \<Longrightarrow> n = objBits sc' - minSchedContextBits"
   by (clarsimp simp: sc_relation_def objBits_simps valid_sched_context_size_def scBits_simps)
 
-lemma state_relation_sc_update:
+(* FIXME RT: Move to Lib *)
+lemma last_take:
+  "\<lbrakk>ls \<noteq> []; 0 < n; n \<le>  length ls\<rbrakk> \<Longrightarrow>last (take n ls) = ls ! (n - 1)"
+  by (induct ls arbitrary: n; fastforce simp: take_Cons nth_Cons split: nat.splits)
+
+lemma take_drop_nth:
+  "\<lbrakk> 0 < n; n < length ls\<rbrakk> \<Longrightarrow> take 1 (drop n ls) = [ls ! n]"
+  apply (induct ls arbitrary: n; clarsimp simp: drop_Cons nth_Cons)
+  by (case_tac n; simp add: drop_Suc_nth)
+
+(* wrap_slice *)
+lemma wrap_slice_start_0:
+  "\<lbrakk>0 < count; mx \<le> length ls; count \<le> mx\<rbrakk> \<Longrightarrow> wrap_slice 0 count mx ls = take count ls"
+  by (clarsimp simp: wrap_slice_def)
+
+lemma butlast_wrap_slice:
+  "\<lbrakk>0 < count; start < mx; count \<le> mx; mx \<le> length list\<rbrakk> \<Longrightarrow>
+   butlast (wrap_slice start count mx list) =  wrap_slice start (count -1) mx list"
+  by (case_tac "start + count - 1 < mx"; clarsimp simp: wrap_slice_def butlast_conv_take add_ac)
+
+lemma last_wrap_slice:
+  "\<lbrakk>0 < count; start < mx; count \<le> mx; mx \<le> length list\<rbrakk>
+   \<Longrightarrow> last (wrap_slice start count mx list)
+           = list ! (if start + count - 1 < mx then start + count - 1 else start + count - mx -1)"
+  by (fastforce simp: wrap_slice_def last_take last_append not_le)
+
+lemma tl_wrap_slice:
+  "\<lbrakk>0 < count; mx \<le> length list; start < mx\<rbrakk> \<Longrightarrow>
+   tl (wrap_slice start count mx list) = wrap_slice (start + 1) (count - 1) mx list"
+  by (fastforce simp: wrap_slice_def tl_take tl_drop drop_Suc)
+
+lemma wrap_slice_max[simp]:
+  "wrap_slice start count start list = take count list"
+  by (clarsimp simp: wrap_slice_def)
+
+lemma length_refills_map[simp]:
+  "\<lbrakk> mx \<le> length list; count \<le> mx \<rbrakk> \<Longrightarrow> length (refills_map start count mx list) = count"
+  by (clarsimp simp: refills_map_def)
+
+(* updateAt *)
+(* FIXME RT: add [simp] *)
+declare length_updateAt[simp]
+declare length_replaceAt[simp]
+
+lemma updateAt_index:
+  "\<lbrakk>xs \<noteq> []; i < length xs; j < length xs\<rbrakk>
+   \<Longrightarrow> (updateAt i xs f) ! j = (if i = j then f (xs ! i) else (xs ! j))"
+  by (fastforce simp: updateAt_def null_def nth_append)
+
+lemma wrap_slice_updateAt_eq:
+  "\<lbrakk>if start + count \<le> mx
+       then (i < start \<or> start + count \<le> i)
+       else (start + count - mx \<le> i \<and> i < start);
+    count \<le> mx; start < mx; mx \<le> length xs; xs \<noteq> []; i < mx\<rbrakk>
+   \<Longrightarrow> wrap_slice start count mx xs = wrap_slice start count mx (updateAt i xs new)"
+  apply (rule nth_equalityI)
+   apply clarsimp
+  by (subst wrap_slice_index; clarsimp simp: updateAt_index split: if_split_asm)+
+
+lemma take_updateAt_eq[simp]:
+  "n \<le> i \<Longrightarrow> take n (updateAt i ls f) = take n ls" 
+  by (clarsimp simp: updateAt_def)
+
+lemma valid_obj'_scPeriod_update[simp]:
+  "valid_obj' (KOSchedContext (scPeriod_update (\<lambda>_. period) sc')) = valid_obj' (KOSchedContext sc')"
+  by (fastforce simp: valid_obj'_def valid_sched_context'_def valid_sched_context_size'_def objBits_simps)
+
+(* should all wp rules for valid_objs/valid_objs' be in this form? *)
+lemma updateSchedContext_valid_objs'[wp]:
+  "\<lbrace>valid_objs' and
+    (\<lambda>s. ((\<lambda>sc'. valid_obj' (injectKOS sc') s \<longrightarrow> valid_obj' (injectKOS (f' sc')) s)
+              |< scs_of' s) scp)\<rbrace>
+    updateSchedContext scp f'
+   \<lbrace>\<lambda>_. valid_objs'\<rbrace>"
+  apply (wpsimp simp: updateSchedContext_def wp: set_sc'.valid_objs')
+  by (fastforce simp: valid_obj'_def valid_sched_context'_def valid_sched_context_size'_def
+                      obj_at'_def projectKOs scBits_simps objBits_simps opt_map_left_Some)
+
+lemma updateSchedContext_obj_at'[wp]:
+  "\<forall>sc'. objBits sc' = objBits (f' sc'::sched_context) \<Longrightarrow>
+   updateSchedContext scp f' \<lbrace>\<lambda>s. P (sc_at' p s)\<rbrace>"
+  apply (wpsimp simp: updateSchedContext_def wp: set_sc'.set_wp)
+  apply (clarsimp simp: obj_at'_def ps_clear_upd projectKOs objBits_simps)
+  done
+
+(* it would be good to rewrite all update wp rules in this form *)
+lemma updateSchedContext_wp:
+  "\<lbrace> \<lambda>s. sc_at' sc_ptr s \<longrightarrow>
+       Q (s\<lparr>ksPSpace := ksPSpace s(sc_ptr \<mapsto> KOSchedContext (f' (the (scs_of' s sc_ptr))))\<rparr>) \<rbrace>
+   updateSchedContext sc_ptr f'
+   \<lbrace> \<lambda>rv. Q \<rbrace>"
+  by (wpsimp simp: updateSchedContext_def wp: set_sc'.set_wp)
+     (clarsimp simp: obj_at'_def projectKOs opt_map_left_Some elim!: rsubst[where P=Q])
+
+lemma no_fail_setSchedContext[wp]:
+  "no_fail (sc_at' ptr and (\<lambda>s'. pred_map (\<lambda>k::sched_context. objBits k = objBits new) (scs_of' s') ptr)) (setSchedContext ptr new)"
+  unfolding setSchedContext_def by (wpsimp simp: pred_map_simps obj_at'_def projectKOs)
+
+lemma no_fail_updateSchedContext[wp]:
+  "no_fail (sc_at' ptr and (\<lambda>s'. pred_map (\<lambda>k::sched_context. objBits k = objBits (f k)) (scs_of' s') ptr))
+         (updateSchedContext ptr f)"
+  by (wpsimp simp: updateSchedContext_def obj_at'_def projectKOs pred_map_simps opt_map_Some)
+
+(* rewrite rules for updateSchedCOntext *)
+lemma updateSchedContext_decompose:
+   "monadic_rewrite False True
+     (sc_at' scPtr and K (\<forall>sc. objBits (f sc) = objBits sc) and K (\<forall>sc. objBits (g sc) = objBits sc))
+     (updateSchedContext scPtr (g o f))
+     (do updateSchedContext scPtr f;
+         updateSchedContext scPtr g
+      od)"
+  unfolding updateSchedContext_def bind_assoc o_def
+  using getSchedContext_setSchedContext_decompose by blast
+
+lemma updateSchedContext_decompose_twice:
+  "\<lbrakk>\<forall>sc. objBits (f sc) = objBits sc; \<forall>sc. objBits (g sc) = objBits sc;
+    \<forall>sc. objBits (h sc) = objBits sc\<rbrakk> \<Longrightarrow>
+    monadic_rewrite False True
+     (sc_at' scPtr)
+     (updateSchedContext scPtr (h o g o f))
+     (do updateSchedContext scPtr f;
+         updateSchedContext scPtr g;
+         updateSchedContext scPtr h
+      od)"
+  apply (rule monadic_rewrite_imp)
+   apply (rule monadic_rewrite_trans)
+    apply (rule updateSchedContext_decompose)
+   apply (rule monadic_rewrite_bind_tail)
+    apply simp
+    apply (rule updateSchedContext_decompose[simplified])
+   apply (wpsimp wp: updateSchedContext_wp)
+  apply (clarsimp simp: obj_at_simps opt_map_def ps_clear_upd)
+  done
+
+lemma updateSchedContext_decompose_thrice:
+  "\<lbrakk>\<forall>sc. objBits (f sc) = objBits sc; \<forall>sc. objBits (g sc) = objBits sc;
+    \<forall>sc. objBits (h sc) = objBits sc;  \<forall>sc. objBits (k sc) = objBits sc\<rbrakk> \<Longrightarrow>
+    monadic_rewrite False True
+     (sc_at' scPtr)
+     (updateSchedContext scPtr (k o h o g o f))
+     (do updateSchedContext scPtr f;
+         updateSchedContext scPtr g;
+         updateSchedContext scPtr h;
+         updateSchedContext scPtr k
+      od)"
+  apply (rule monadic_rewrite_imp)
+   apply (rule monadic_rewrite_trans)
+    apply (rule updateSchedContext_decompose)
+   apply (rule monadic_rewrite_bind_tail)
+    apply simp
+    apply (rule updateSchedContext_decompose_twice[simplified]; simp)
+   apply (wpsimp wp: updateSchedContext_wp)
+  apply (clarsimp simp: obj_at_simps ps_clear_upd opt_map_def)
+  done
+
+(* projection project *)
+
+(* it would be good to rewrite all getting wp rules in this form *)
+lemma getSchedContext_wp':
+  "\<lbrace>\<lambda>s. sc_at' p s  \<longrightarrow> P (the (scs_of' s p)) s\<rbrace> getSchedContext p \<lbrace>P\<rbrace>"
+  by (wpsimp simp: obj_at'_def projectKOs opt_map_left_Some)
+
+lemma is_active_sc'_cross:
+  assumes p: "pspace_relation (kheap s) (ksPSpace s')"
+  assumes t: "is_active_sc2 ptr s"
+  shows "is_active_sc' ptr s'"
+  using assms
+  supply projection_rewrites[simp]
+  apply (clarsimp simp: projectKOs is_active_sc2_def is_active_sc'_def
+                 split: option.split_asm Structures_A.kernel_object.split_asm)
+  apply (drule (1) pspace_relation_absD, clarsimp split: if_split_asm)
+  by (case_tac z; simp add: sc_relation_def)
+
+lemma set_refills_is_active_sc2[wp]:
+  "set_refills ptr new \<lbrace>is_active_sc2 ptr'\<rbrace>"
+  apply (wpsimp simp: is_active_sc2_def wp: set_refills_wp)
+  by (clarsimp simp: obj_at_def opt_map_def)
+
+lemma ovalid_readRefillReady'[rule_format, simp]:
+  "ovalid (\<lambda>s. sc_at' scp s \<longrightarrow> P (((\<lambda>sc'. rTime (refillHd sc') \<le> ksCurTime s + kernelWCETTicks) |< scs_of' s) scp) s)
+              (readRefillReady scp) P"
+  unfolding readRefillReady_def readSchedContext_def ovalid_def
+  by (fastforce simp: obind_def opt_map_left_Some obj_at'_def projectKOs
+                dest: use_ovalid[OF ovalid_readCurTime]
+               dest!: readObject_misc_ko_at'
+               split: option.split_asm)+
+
+lemma refillReady_wp':
+  "\<lbrace>\<lambda>s. sc_at' scp s \<longrightarrow> P (((\<lambda>sc'. rTime (refillHd sc') \<le> ksCurTime s + kernelWCETTicks) |< scs_of' s) scp) s\<rbrace>
+    refillReady scp \<lbrace>P\<rbrace>"
+  unfolding refillReady_def
+  by wpsimp (drule use_ovalid[OF ovalid_readRefillReady'])
+
+(* end : projection project *)
+
+lemma state_relation_sc_update':
   assumes
-      R1: "\<forall>sc n sc'. P sc \<longrightarrow> P' sc' \<longrightarrow> sc_relation sc n sc' \<longrightarrow> sc_relation (f sc) n (f' sc')"
-  and R2: "\<forall>sc sc' s'. P sc \<longrightarrow> P' sc' \<longrightarrow> heap_ls (replyPrevs_of s') (scReply sc') (sc_replies sc)
-                         \<longrightarrow> heap_ls (replyPrevs_of s') (scReply (f' sc')) (sc_replies (f sc))"
+      R1: "\<forall>s s'. (s, s') \<in> state_relation \<longrightarrow>
+         P s \<longrightarrow> P' s' \<longrightarrow> sc_at ptr s \<longrightarrow> sc_at' ptr s' \<longrightarrow>
+           (\<forall>n. (((\<lambda>ko. obj_bits ko = min_sched_context_bits + n) |< kheap s) ptr) \<longrightarrow>
+           sc_relation (the ((scs_of2 s ||> f) ptr)) n (the ((scs_of' s' ||> f') ptr)))"
+  and R2: "\<forall>s s'. (s, s') \<in> state_relation \<longrightarrow>                
+         P s \<longrightarrow> P' s' \<longrightarrow> sc_at ptr s \<longrightarrow> sc_at' ptr s' \<longrightarrow>
+           heap_ls (replyPrevs_of s')  (scReply (the ((scs_of' s' ||> f') ptr)))
+             (sc_replies (the ((scs_of2 s ||> f) ptr)))"
   and sz: "\<forall>sc'::sched_context. objBits sc' = objBits (f' sc')"
   shows
-  "\<lbrakk>(s, s') \<in> state_relation; sc_at ptr s; sc_at' ptr s';
-    P (the ((kheap s |> sc_of) ptr)); P' (the (scs_of' s' ptr))\<rbrakk> \<Longrightarrow>
+  "\<lbrakk>(s, s') \<in> state_relation; P s; P' s'; sc_at ptr s; sc_at' ptr s'\<rbrakk> \<Longrightarrow>
      (kheap_update (\<lambda>hp p. if p = ptr
                            then
                              case hp ptr of
@@ -406,6 +605,7 @@ lemma state_relation_sc_update:
                                      \<Rightarrow> Some (KOSchedContext (f' sc'))
                                  | _ \<Rightarrow> hp' ptr
                                 else hp' p)) s') \<in> state_relation"
+  supply projection_rewrites[simp]
   proof -
   have z': "\<And>s. sc_at' ptr s
                \<Longrightarrow> \<forall>sc'::sched_context. map_to_ctes ((\<lambda>hp' p. if p = ptr then case hp' ptr of
@@ -418,15 +618,17 @@ lemma state_relation_sc_update:
   have S: "\<And>(v::'a::pspace_storable). (1 :: word32) < 2 ^ (objBits v)"
     by (clarsimp simp: obj_at_simps objBits_defs pteBits_def pdeBits_def scBits_pos_power2
                 split: kernel_object.splits arch_kernel_object.splits)
-  assume H: "(s, s') \<in> state_relation" "sc_at ptr s" "sc_at' ptr s'"
-  and   H': "P (the ((kheap s |> sc_of) ptr))"
-            "P' (the (scs_of' s' ptr))"
+  assume H: "(s, s') \<in> state_relation" "P s" "P' s'" "sc_at ptr s" "sc_at' ptr s'"
   show ?thesis
-    using H H' S assms
+    using H S sz
+  apply -
+    apply (insert R1[rule_format, OF H(1) H(2) H(3) H(4) H(5)]
+                  R2[rule_format, OF H(1) H(2) H(3) H(4) H(5)])
     apply (clarsimp simp: state_relation_def)
     apply (clarsimp simp: obj_at_def is_sc_obj)
+    apply (drule_tac x=n in meta_spec, clarsimp)
     apply (prop_tac "obj_at (same_caps (kernel_object.SchedContext _ n)) ptr s")
-     apply (clarsimp simp: obj_at_def)
+     apply (clarsimp simp: obj_at_def obj_bits_def)
     apply (clarsimp simp: obj_at'_def projectKOs fun_upd_def[symmetric]
                           z[simplified obj_at'_def projectKO_eq projectKO_opts_defs])
     apply (rename_tac n sc sc')
@@ -441,22 +643,18 @@ lemma state_relation_sc_update:
      apply (frule bspec, erule domI)
      apply (rule ballI, drule(1) bspec)
      apply (drule domD)
-     apply (clarsimp simp: project_inject opt_map_left_Some sc_of_def
+     apply (clarsimp simp: project_inject  
                     split: if_split_asm kernel_object.split_asm)
-     apply (drule_tac x=sc in spec)+
-     apply clarsimp
-    apply (drule_tac x=n and y=sc' in spec2)
-     apply (drule_tac x=sc' in spec)+
-     apply clarsimp
+     apply (drule_tac x=sc' in spec)
      apply (rename_tac bb aa ba)
      apply (drule_tac x="(aa, ba)" in bspec, simp)
      apply (clarsimp simp: objBits_def)
      apply (frule_tac ko'="kernel_object.SchedContext sc n" and x'=ptr in obj_relation_cut_same_type)
         apply simp+
      apply (erule obj_relation_cutsE)
-            apply (simp split: if_split_asm)+
+            apply ((simp split: if_split_asm)+)[8]
     (* sc_replies_relation *)
-    apply (frule (1) sc_replies_relation_prevs_list')
+    apply (frule (1) sc_replies_relation_prevs_list'[simplified])
     apply (subst replyPrevs_of_non_reply_update[simplified]; (simp add: typ_at'_def ko_wp_at'_def)?)
     apply (simp add: sc_replies_relation_def)
     apply (clarsimp simp: vs_all_heap_simps sc_replies_of_scs_def map_project_def opt_map_left_Some)
@@ -485,41 +683,20 @@ lemma state_relation_sc_update:
     done
 qed
 
-lemma updateSchedContext_decompose:
-   "monadic_rewrite False True
-     (sc_at' scPtr and K (\<forall>sc. objBits (f sc) = objBits sc) and K (\<forall>sc. objBits (g sc) = objBits sc))
-     (updateSchedContext scPtr (g o f))
-     (do updateSchedContext scPtr f;
-         updateSchedContext scPtr g
-      od)"
-  unfolding updateSchedContext_def bind_assoc o_def
-  using getSchedContext_setSchedContext_decompose by blast
-
-lemma updateSchedContext_wp:
-  "\<lbrace> \<lambda>s. \<forall>sc'::sched_context. ko_at' sc' sc_ptr s
-                \<longrightarrow> Q (s\<lparr>ksPSpace := ksPSpace s(sc_ptr \<mapsto> KOSchedContext (f' sc'))\<rparr>) \<rbrace>
-   updateSchedContext sc_ptr f'
-   \<lbrace> \<lambda>rv. Q \<rbrace>"
-  by (wpsimp simp: updateSchedContext_def wp: set_sc'.set_wp)
-
-lemma no_fail_setSchedContext[wp]:
-  "no_fail (sc_at' ptr and (\<lambda>s'. pred_map (\<lambda>k::sched_context. objBits k = objBits new) (scs_of' s') ptr)) (setSchedContext ptr new)"
-  unfolding setSchedContext_def by (wpsimp simp: pred_map_simps obj_at'_def projectKOs)
-
-lemma no_fail_updateSchedContext[wp]:
-  "no_fail (sc_at' ptr and (\<lambda>s'. pred_map (\<lambda>k::sched_context. objBits k = objBits (f k)) (scs_of' s') ptr))
-         (updateSchedContext ptr f)"
-  by (wpsimp simp: updateSchedContext_def obj_at'_def projectKOs pred_map_simps opt_map_Some)
-
-lemma updateSchedContext_corres_gen:
+lemma updateSchedContext_corres_gen':
   assumes
-      R1: "\<forall>sc n sc'. P sc \<longrightarrow> P' sc' \<longrightarrow> sc_relation sc n sc' \<longrightarrow> sc_relation (f sc) n (f' sc')"
-  and R2: "\<forall>sc sc' s'. P sc \<longrightarrow> P' sc' \<longrightarrow> heap_ls (replyPrevs_of s') (scReply sc') (sc_replies sc)
-                         \<longrightarrow> heap_ls (replyPrevs_of s') (scReply (f' sc')) (sc_replies (f sc))"
+      R1: "\<forall>s s'. (s, s') \<in> state_relation \<longrightarrow>
+           P s \<longrightarrow> P' s' \<longrightarrow> sc_at ptr s \<longrightarrow> sc_at' ptr s' \<longrightarrow>
+           (\<forall>n. (((\<lambda>ko. obj_bits ko = min_sched_context_bits + n) |< kheap s) ptr)\<longrightarrow>
+           sc_relation (the ((scs_of2 s ||> f) ptr)) n (the ((scs_of' s' ||> f') ptr)))"
+  and R2: "\<forall>s s'. (s, s') \<in> state_relation \<longrightarrow>                
+          P s \<longrightarrow> P' s' \<longrightarrow> sc_at ptr s \<longrightarrow> sc_at' ptr s' \<longrightarrow>
+           heap_ls (replyPrevs_of s')  (scReply (the ((scs_of' s' ||> f') ptr)))
+             (sc_replies (the ((scs_of2 s ||> f) ptr)))"
   and sz: "\<forall>sc'::sched_context. objBits sc' = objBits (f' sc')"
   shows "corres dc
-         (sc_at ptr and (\<lambda>s. P (the ((kheap s |> sc_of) ptr))))
-         (sc_at' ptr and (\<lambda>s'. P' (the (scs_of' s' ptr))))
+         (sc_at ptr and P)
+         (sc_at' ptr and P')
             (update_sched_context ptr f)
             (updateSchedContext ptr f')"
   unfolding corres_underlying_def using sz
@@ -535,9 +712,9 @@ lemma updateSchedContext_corres_gen:
    apply (rule_tac x="((), s\<lparr>kheap := kheap s(ptr \<mapsto>
                   kernel_object.SchedContext (f sc) n)\<rparr>)" in bexI)
     apply clarsimp
-    apply (drule state_relation_sc_update[OF R1 R2 sz, simplified])
+    apply (drule state_relation_sc_update'[OF R1 R2 sz, simplified])
       apply ((fastforce simp: obj_at_def is_sc_obj obj_at'_def projectKOs)+)[4]
-    apply (clarsimp simp: obj_at_def obj_at'_def projectKOs fun_upd_def
+    apply (clarsimp simp: obj_at_def obj_at'_def projectKOs fun_upd_def opt_map_left_Some
                     cong: abstract_state.ext_split)
     apply (clarsimp cong: kernel_state.ext_split)
    apply (clarsimp simp: update_sched_context_def obj_at_def in_monad
@@ -546,44 +723,39 @@ lemma updateSchedContext_corres_gen:
                     simp: obj_at'_def pred_map_simps projectKOs opt_map_simps)
   done
 
-lemmas updateSchedContext_corres = updateSchedContext_corres_gen[where P=\<top> and P'=\<top>, simplified]
+lemmas updateSchedContext_corres = updateSchedContext_corres_gen'[where P=\<top> and P'=\<top>, simplified]
 
 lemma refillAddTail_corres:
   "time = time' \<and> amount = amount'
    \<Longrightarrow> corres dc (sc_at sc_ptr)
-                 (obj_at' (\<lambda>sc'. scRefillHead sc' < scRefillMax sc' \<and> 0 < scRefillCount sc'
-                                 \<and> scRefills sc' \<noteq> [] \<and> scRefillCount sc' < scRefillMax sc'
-                                 \<and> scRefillMax sc' \<le> length (scRefills sc')) sc_ptr)
+                 (sc_at' sc_ptr and
+                  (\<lambda>s'. ((\<lambda>sc'. scRefillCount sc' < scRefillMax sc' \<and> std_sc' sc') |< scs_of' s') sc_ptr))
                  (refill_add_tail sc_ptr \<lparr>r_time = time, r_amount = amount\<rparr>)
                  (refillAddTail sc_ptr (Refill time' amount'))"
+  supply projection_rewrites[simp]
   apply (clarsimp simp: refill_add_tail_def refillAddTail_def getRefillNext_getSchedContext
                         getRefillSize_def2 liftM_def get_refills_def)
   apply (rule corres_symb_exec_r[OF _ get_sc_sp', rotated]; (solves wpsimp)?)+
   apply (rename_tac sc')
   apply (rule corres_guard_imp)
     apply (rule corres_assert_assume_r)
-    apply (rule updateSchedContext_corres_gen[where P=\<top> and P'="\<lambda>sc'. scRefillHead sc' < scRefillMax sc' \<and>
-                             0 < scRefillCount sc' \<and>
-                             scRefills sc' \<noteq> [] \<and>
-                             scRefillCount sc' < scRefillMax sc' \<and>
-                             scRefillMax sc' \<le> length (scRefills sc')"])
-      apply (clarsimp simp: sc_relation_def length_replaceAt)
+    apply (rule updateSchedContext_corres_gen'[where P=\<top>
+                and P'="(\<lambda>s'. ((\<lambda>sc'. scRefillCount sc' < scRefillMax sc' \<and> std_sc' sc') |< scs_of' s') sc_ptr)"])
+      apply (clarsimp, drule (3) state_relation_sc_relation)
+      apply (clarsimp simp: obj_at_simps is_sc_obj)
+      apply (rename_tac sc')
+      apply (clarsimp simp: sc_relation_def neq_Nil_lengthI)
+      apply (prop_tac "scRefills sc' \<noteq> []")
+       apply (clarsimp simp: neq_Nil_lengthI)
       apply (clarsimp simp: refills_map_def)
-      apply (subst wrap_slice_append)
-         apply simp
-        apply simp
-       apply (simp add: length_replaceAt)
+      apply (subst wrap_slice_append; simp)
       apply (insert less_linear)[1]
       apply (drule_tac x="scRefillMax sc'" and y="scRefillHead sc' + scRefillCount sc' + Suc 0" in meta_spec2)
       apply (erule disjE)
        apply (simp add: refillNextIndex_def refillTailIndex_def Let_def)
-       apply (intro conjI impI; clarsimp simp: Suc_diff_Suc wrap_slice_replaceAt_eq)
-          apply (clarsimp simp: nat_le_Suc_less)
-          apply (metis add_less_mono add_less_mono1 le_refl le_simps(1) mult_is_add.mult_commute nat_diff_less wrap_slice_replaceAt_eq)
-         apply (clarsimp simp: replaceAt_index refill_map_def)
-        apply (clarsimp simp: eq_diff_iff not_le)
-        apply (metis add.commute add_gr_0 less_add_same_cancel1 less_or_eq_imp_le wrap_slice_replaceAt_eq)
-       apply (clarsimp simp: replaceAt_index refill_map_def)
+       apply (intro conjI impI;
+              clarsimp simp: Suc_diff_Suc wrap_slice_replaceAt_eq[symmetric] neq_Nil_lengthI
+                             nat_le_Suc_less refill_map_def replaceAt_index)
       apply (erule disjE)
        apply clarsimp
        apply (rule conjI)
@@ -596,13 +768,14 @@ lemma refillAddTail_corres:
       apply (rule conjI)
        apply (clarsimp simp: refillNextIndex_def refillTailIndex_def Let_def)
        apply (intro conjI impI; (clarsimp simp: not_le wrap_slice_replaceAt_eq)?)
-       apply (metis add_leE le_refl le_simps(1) less_SucI mult_is_add.mult_commute nat_neq_iff not_less_eq trans_less_add2 wrap_slice_replaceAt_eq)
+       apply (metis add_leE le_refl le_simps(1) less_SucI mult_is_add.mult_commute nat_neq_iff
+                    not_less_eq trans_less_add2 wrap_slice_replaceAt_eq)
       apply (clarsimp simp: refillNextIndex_def refillTailIndex_def Let_def not_le)
       apply (clarsimp simp: replaceAt_index refill_map_def)
-     apply fastforce
-    apply (clarsimp simp: objBits_simps length_replaceAt)
+     apply (fastforce simp: obj_at_simps is_sc_obj dest!: state_relation_sc_replies_relation_sc)
+    apply (clarsimp simp: objBits_simps)
    apply (clarsimp simp: obj_at_def is_sc_obj)
-  apply (clarsimp simp: obj_at'_def projectKOs opt_map_def)
+  apply (clarsimp simp: obj_at'_def projectKOs)
   done
 
 lemma isRoundRobin_sp:
@@ -618,30 +791,28 @@ lemma isRoundRobin_sp:
 
 lemma maybeAddEmptyTail_corres:
   "corres dc
-          (is_active_sc sc_ptr)
-          (\<lambda>s'. obj_at' (\<lambda>sc'. scRefillHead sc' < scRefillMax sc' \<and> 0 < scRefillCount sc'
-                                \<and> scRefills sc' \<noteq> [] \<and> scRefillCount sc' < scRefillMax sc'
-                                \<and> scRefillMax sc' \<le> length (scRefills sc')) sc_ptr s')
+          (is_active_sc2 sc_ptr)
+                 (sc_at' sc_ptr and
+                  (\<lambda>s'. ((\<lambda>sc'. scRefillCount sc' < scRefillMax sc' \<and> std_sc' sc') |< scs_of' s') sc_ptr))
           (maybe_add_empty_tail sc_ptr)
           (maybeAddEmptyTail sc_ptr)" (is "corres _ ?abs ?conc _ _")
-  apply (rule corres_guard_imp[where Q="?abs" and Q'="?conc and sc_at' sc_ptr", rotated];
-         clarsimp simp add: obj_at'_def projectKOs)
+  supply projection_rewrites[simp]
   apply (rule corres_cross_add_abs_guard[where Q="sc_at sc_ptr"])
-   apply (fastforce simp: dest!: sc_at'_cross[OF state_relation_pspace_relation])
+   apply (fastforce dest!: sc_at'_cross[OF state_relation_pspace_relation])
   apply (clarsimp simp: maybe_add_empty_tail_def maybeAddEmptyTail_def get_refills_def)
   apply (rule corres_split'[rotated 2, OF is_round_robin_sp isRoundRobin_sp])
    apply (corressimp corres: isRoundRobin_corres)
-  apply (clarsimp simp: obj_at_def is_sc_obj vs_all_heap_simps)
+  apply (clarsimp simp: obj_at_def is_sc_obj)
   apply (clarsimp simp: when_def)
   apply (rule corres_split'[rotated 2, OF get_sched_context_sp get_sc_sp'])
    apply (corressimp corres: get_sc_corres)
    apply (fastforce intro: valid_objs_valid_sched_context_size
-                     simp: obj_at_def is_sc_obj_def vs_all_heap_simps)
+                     simp: obj_at_def is_sc_obj_def)
   apply (rename_tac sc')
   apply (corressimp corres: refillAddTail_corres)
   apply (frule refill_hd_relation; clarsimp simp: obj_at'_def projectKOs)
   apply (fastforce dest: valid_objs_valid_sched_context_size
-                   simp: obj_at_def is_sc_obj_def vs_all_heap_simps refill_map_def)
+                   simp: obj_at_def is_sc_obj_def refill_map_def)
   done
 
 lemma getRefills_sp:
@@ -655,54 +826,9 @@ lemma getRefills_sp:
   apply (clarsimp simp: obj_at'_def projectKOs)
   done
 
-lemma updateAt_index:
-  "\<lbrakk>xs \<noteq> []; i < length xs; j < length xs\<rbrakk>
-   \<Longrightarrow> (updateAt i xs f) ! j = (if i = j then f (xs ! i) else (xs ! j))"
-  by (fastforce simp: updateAt_def null_def nth_append)
-
-(* FIXME RT: move *)
-lemma active_sc_at_cross:
-  assumes p: "pspace_relation (kheap s) (ksPSpace s')"
-  assumes ps: "pspace_aligned s" "pspace_distinct s"
-  assumes t: "active_sc_at ptr s"
-  shows "active_sc_at' ptr s'"
-  using assms
-  apply (clarsimp simp: active_sc_at_def active_sc_at'_def projectKOs active_sc_def)
-  apply (drule (1) pspace_relation_absD, clarsimp split: if_split_asm)
-  apply (case_tac z; simp add: sc_relation_def)
-  by (fastforce dest!: aligned_distinct_ko_at'I[where 'a=sched_context] elim: obj_at'_weakenE)
-
-(* FIXME RT: add [simp] *)
-declare length_updateAt[simp]
-
-lemma wrap_slice_updateAt_eq:
-  "\<lbrakk>if start + count \<le> mx
-       then (i < start \<or> start + count \<le> i)
-       else (start + count - mx \<le> i \<and> i < start);
-    count \<le> mx; start < mx; mx \<le> length xs; xs \<noteq> []; i < mx\<rbrakk>
-   \<Longrightarrow> wrap_slice start count mx xs = wrap_slice start count mx (updateAt i xs new)"
-  apply (rule nth_equalityI)
-   apply clarsimp
-  by (subst wrap_slice_index; clarsimp simp: updateAt_index split: if_split_asm)+
-
-lemma take_updateAt_eq[simp]:
-  "n \<le> i \<Longrightarrow> take n (updateAt i ls f) = take n ls" 
-  by (clarsimp simp: updateAt_def)
-
-lemma tl_wrap_slice:
-  "\<lbrakk>0 < count; mx \<le> length list; start < mx\<rbrakk> \<Longrightarrow>
-   tl (wrap_slice start count mx list) = wrap_slice (start + 1) (count - 1) mx list"
-  by (fastforce simp: wrap_slice_def tl_take tl_drop drop_Suc)
-
-lemma wrap_slice_max[simp]:
-  "wrap_slice start count start list = take count list"
-  by (clarsimp simp: wrap_slice_def)
-
-thm valid_sched_context'_def active_sc_at_equiv
-
 lemma sc_relation_updateRefillHd:
   "\<lbrakk>sc_relation sc n sc'; \<forall>refill'. f (refill_map refill') = refill_map (f' refill');
-        scRefills sc' \<noteq> []; scRefillMax sc' \<le> length (scRefills sc');
+        scRefillMax sc' \<le> length (scRefills sc');
         scRefillHead sc' < scRefillMax sc'; scRefillCount sc' \<le> scRefillMax sc';
         0 < scRefillCount sc'\<rbrakk>
        \<Longrightarrow> sc_relation (sc_refills_update (\<lambda>refills. f (hd refills) # tl refills) sc) n
@@ -713,54 +839,34 @@ lemma sc_relation_updateRefillHd:
   apply (subst hd_Cons_tl[where xs="wrap_slice _ _ _ (updateAt _ _ _)", symmetric])
    apply (clarsimp intro!: neq_Nil_lengthI)
   apply simp
-  apply (subst hd_wrap_slice; (simp add: updateAt_index tl_wrap_slice)?)+
+  apply (subst hd_wrap_slice; (simp add: updateAt_index tl_wrap_slice neq_Nil_lengthI)?)+
   apply (case_tac "Suc (scRefillHead sc') < scRefillMax sc'")
    apply (prop_tac "wrap_slice (Suc (scRefillHead sc')) (scRefillCount sc' - Suc 0)
                  (scRefillMax sc') (updateAt (scRefillHead sc') (scRefills sc') f')
           = wrap_slice (Suc (scRefillHead sc')) (scRefillCount sc' - Suc 0) (scRefillMax sc') (scRefills sc')")
     apply (subst wrap_slice_updateAt_eq[symmetric]; clarsimp)
-     apply fastforce+
+     apply (fastforce simp: neq_Nil_lengthI)+
   apply (clarsimp simp: not_less le_eq_less_or_eq[where m="scRefillMax sc'" for sc'])
   done
 
 lemma updateRefillHd_corres:
-  "\<lbrakk>sc_ptr = scPtr;
-    \<forall>refill refill'. refill = refill_map refill' \<longrightarrow> f refill = (refill_map (f' refill'))\<rbrakk>
+  "\<lbrakk>sc_ptr = scPtr; \<forall>refill refill'. refill = refill_map refill' \<longrightarrow> f refill = (refill_map (f' refill'))\<rbrakk>
    \<Longrightarrow> corres dc
-        (pspace_aligned and pspace_distinct and sc_at sc_ptr and is_active_sc sc_ptr)
-        valid_objs'
+        (sc_at sc_ptr and is_active_sc2 sc_ptr)
+        ((\<lambda>s'. ((\<lambda>sc'. scRefillCount sc' \<le> scRefillMax sc' \<and> std_sc' sc') |< scs_of' s') sc_ptr) and sc_at' sc_ptr)
         (update_refill_hd sc_ptr f)
         (updateRefillHd scPtr f')"
-  apply (rule_tac Q="active_sc_at' sc_ptr" in corres_cross_add_guard)
-   apply (clarsimp simp: active_sc_at_equiv[symmetric])
-   apply (fastforce elim!: active_sc_at_cross[OF state_relation_pspace_relation])
+  supply projection_rewrites[simp]
+  apply (rule_tac Q="is_active_sc' scPtr" in corres_cross_add_guard)
+   apply (fastforce dest!: is_active_sc'_cross[OF state_relation_pspace_relation])
   apply (clarsimp simp: update_refill_hd_def updateRefillHd_def)
   apply (rule corres_guard_imp)
-    apply (rule updateSchedContext_corres_gen[where P=\<top> and P'="\<lambda>sc'. scRefills sc' \<noteq> []
-                      \<and> scRefillMax sc' \<le> length (scRefills sc') \<and>
-                      (scRefillHead sc' < scRefillMax sc' \<and>
-                       scRefillCount sc' \<le> scRefillMax sc' \<and> 0 < scRefillCount sc')"])
-      apply (clarsimp simp: sc_relation_updateRefillHd)
-     apply (clarsimp simp: objBits_simps)+
-  apply (clarsimp simp: active_sc_at'_def)
-  apply (drule obj_at_ko_at', clarsimp)
-  apply (frule (1) sc_ko_at_valid_objs_valid_sc')
-  by (clarsimp simp: obj_at'_def projectKOs opt_map_left_Some valid_sched_context'_def MIN_REFILLS_def)
-
-lemma last_take:
-  "\<lbrakk>ls \<noteq> []; 0 < n; n \<le>  length ls\<rbrakk> \<Longrightarrow>last (take n ls) = ls ! (n - 1)"
-  by (induct ls arbitrary: n; fastforce simp: take_Cons nth_Cons split: nat.splits)
-
-lemma butlast_wrap_slice:
-  "\<lbrakk>0 < count; start < mx; count \<le> mx; mx \<le> length list\<rbrakk> \<Longrightarrow>
-   butlast (wrap_slice start count mx list) =  wrap_slice start (count -1) mx list"
-  by (case_tac "start + count - 1 < mx"; clarsimp simp: wrap_slice_def butlast_conv_take add_ac)
-
-lemma last_wrap_slice:
-  "\<lbrakk>0 < count; start < mx; count \<le> mx; mx \<le> length list\<rbrakk>
-   \<Longrightarrow> last (wrap_slice start count mx list)
-           = list ! (if start + count - 1 < mx then start + count - 1 else start + count - mx -1)"
-  by (fastforce simp: wrap_slice_def last_take last_append not_le)
+    apply (rule updateSchedContext_corres_gen'[where P=\<top>
+      and P'="(\<lambda>s'. ((\<lambda>sc'. scRefillCount sc' \<le> scRefillMax sc' \<and> std_sc' sc') |< scs_of' s') sc_ptr) and is_active_sc' scPtr"])
+      apply (clarsimp, drule (3) state_relation_sc_relation)
+      apply (fastforce simp: is_sc_obj obj_at_simps is_active_sc'_def elim!: sc_relation_updateRefillHd)
+     apply (fastforce simp: obj_at_simps is_sc_obj dest!: state_relation_sc_replies_relation_sc)
+  by (clarsimp simp: objBits_simps)+
 
 lemma sc_relation_updateRefillTl:
   "\<lbrakk> sc_relation sc n sc'; \<forall>refill'. f (refill_map refill') = refill_map (f' refill');
@@ -770,10 +876,8 @@ lemma sc_relation_updateRefillTl:
        \<Longrightarrow> sc_relation
             (sc_refills_update (\<lambda>refills. butlast refills @ [f (last refills)]) sc) n
             (scRefills_update (\<lambda>_. updateAt (refillTailIndex sc') (scRefills sc') f') sc')"
-apply (prop_tac "scRefills sc' \<noteq> []")
-apply fastforce
-
-
+  apply (prop_tac "scRefills sc' \<noteq> []")
+   apply fastforce
   apply (clarsimp simp: sc_relation_def refills_map_def)
   apply (simp add: snoc_eq_iff_butlast)
   apply (prop_tac "wrap_slice (scRefillHead sc') (scRefillCount sc') (scRefillMax sc')
@@ -783,7 +887,6 @@ apply fastforce
               (updateAt (refillTailIndex sc') (scRefills sc') f') \<noteq> []")
    apply (clarsimp intro!: neq_Nil_lengthI)
   apply clarsimp
-
   apply (prop_tac "wrap_slice (scRefillHead sc') (scRefillCount sc' - Suc 0)
              (scRefillMax sc')
              (updateAt (refillTailIndex sc') (scRefills sc') f') = wrap_slice (scRefillHead sc') (scRefillCount sc' - Suc 0)
@@ -802,24 +905,22 @@ lemma updateRefillTl_corres:
   "\<lbrakk>sc_ptr = scPtr;
     \<forall>refill refill'. refill = refill_map refill' \<longrightarrow> f refill = (refill_map (f' refill'))\<rbrakk>
    \<Longrightarrow> corres dc
-              (pspace_aligned and pspace_distinct and sc_at sc_ptr and active_sc_at sc_ptr)
-              valid_objs'
+              (sc_at sc_ptr and is_active_sc2 sc_ptr)
+              (sc_at' scPtr and valid_objs')
               (update_refill_tl sc_ptr f)
               (updateRefillTl scPtr f')"
-  apply (rule_tac Q="active_sc_at' sc_ptr" in corres_cross_add_guard)
-   apply (fastforce simp: active_sc_at_equiv[symmetric] elim!: active_sc_at_cross[OF state_relation_pspace_relation])
+  supply projection_rewrites[simp]
+  apply (rule_tac Q="is_active_sc' scPtr" in corres_cross_add_guard)
+   apply (fastforce dest!: is_active_sc'_cross[OF state_relation_pspace_relation])
   apply (clarsimp simp: update_refill_tl_def updateRefillTl_def)
   apply (rule corres_guard_imp)
-    apply (rule updateSchedContext_corres_gen[where P=\<top> and P'="\<lambda>sc'.
-     scRefillMax sc' \<le> length (scRefills sc') \<and>
-    (scRefillHead sc' < scRefillMax sc' \<and>
-     scRefillCount sc' \<le> scRefillMax sc' \<and> 0 < scRefillCount sc')"])
+    apply (rule updateSchedContext_corres_gen'[where P=\<top> and P'="valid_objs' and is_active_sc' scPtr"])
+      apply (clarsimp, drule (3) state_relation_sc_relation)
+      apply (clarsimp simp: is_sc_obj obj_at_simps is_active_sc'_def)
+      apply (erule (1) valid_objsE', clarsimp simp: valid_obj'_def valid_sched_context'_def)
       apply (clarsimp simp: sc_relation_updateRefillTl)
-     apply (clarsimp simp: objBits_simps)+
-  apply (clarsimp simp: active_sc_at'_def)
-  apply (drule obj_at_ko_at', clarsimp)
-  apply (frule (1) sc_ko_at_valid_objs_valid_sc')
-  by (clarsimp simp: obj_at'_def projectKOs opt_map_left_Some valid_sched_context'_def MIN_REFILLS_def)
+     apply (fastforce simp: obj_at_simps is_sc_obj dest!: state_relation_sc_replies_relation_sc)
+  by (clarsimp simp: objBits_simps)+
 
 lemma getCurSc_sp:
   "\<lbrace>P\<rbrace>
@@ -843,88 +944,36 @@ lemma active_sc_at'_cross:
 
 lemma refillBudgetCheckRoundRobin_corres:
   "corres dc
-          (\<lambda>s. pspace_aligned s \<and> pspace_distinct s \<and> active_sc_valid_refills s \<and> cur_sc_active s
-               \<and> valid_objs s)
-          valid_objs'
+          (cur_sc_active and (\<lambda>s. sc_at (cur_sc s) s))
+          (valid_objs' and (\<lambda>s'. sc_at' (ksCurSc s') s'))
           (refill_budget_check_round_robin usage) (refillBudgetCheckRoundRobin usage)"
+  supply projection_rewrites[simp]
+  apply (subst is_active_sc_rewrite)
   apply (clarsimp simp: refill_budget_check_round_robin_def refillBudgetCheckRoundRobin_def)
   apply (rule corres_split'[rotated 2, OF gets_sp getCurSc_sp])
    apply (corressimp corres: getCurSc_corres)
-
-  apply (rule_tac Q="\<lambda>s. active_sc_at' (ksCurSc s) s" in corres_cross_add_guard)
-   apply (rule_tac sc_ptr="ksCurSc s'" in active_sc_at'_cross, simp+)
-    apply (fastforce dest: valid_objs_valid_sched_context_size )
-   apply (fastforce dest: valid_objs_valid_sched_context_size
-                    simp: vs_all_heap_simps obj_at_def is_sc_obj_def)
-
-  apply (rule_tac Q="\<lambda>_ s. pspace_aligned s \<and> pspace_distinct s \<and> cur_sc_active s \<and> sc_at scPtr s
-                           \<and> cur_sc s = scPtr \<and> sc_refills_sc_at (\<lambda>refills. refills \<noteq> []) scPtr s"
-              and Q'="\<lambda>_ s. valid_objs' s"
-               in corres_split'[rotated 2])
-     apply ((wpsimp wp: get_refills_wp simp: update_refill_hd_rewrite | wpsimp wp: set_refills_wp)+)[1]
-     apply (fastforce intro: valid_objs_valid_sched_context_size
-                       simp: obj_at_def is_sc_obj_def sc_at_pred_n_def vs_all_heap_simps)
-
-    apply (wpsimp wp: updateRefillHd_valid_objs')
-   apply (rule corres_guard_imp)
-     apply (rule_tac f="\<lambda>refill. refill\<lparr>r_amount := r_amount refill - usage\<rparr>"
-                 and f'="\<lambda>r. rAmount_update (\<lambda>_. rAmount r - usage) r"
-                  in updateRefillHd_corres)
-      apply simp
-     apply (clarsimp simp: refill_map_def)
-    apply (fastforce intro: valid_objs_valid_sched_context_size
-                      simp: active_sc_valid_refills_def valid_refills_def vs_all_heap_simps
-                            rr_valid_refills_def obj_at_kh_kheap_simps is_sc_obj_def)
-   apply simp
+  apply (rule_tac Q="\<lambda>s. is_active_sc' (ksCurSc s) s" in corres_cross_add_guard)
+   apply (rule_tac ptr="ksCurSc s'" in is_active_sc'_cross[OF state_relation_pspace_relation]; simp)
+   apply clarsimp
   apply (rule corres_guard_imp)
-    apply (rule_tac f="\<lambda>refill. refill\<lparr>r_amount := r_amount refill + usage\<rparr>"
-                and f'="\<lambda>r. rAmount_update (\<lambda>_. rAmount r + usage) r"
-                 in updateRefillTl_corres)
-     apply simp
-    apply (clarsimp simp: refill_map_def)
-   apply (clarsimp simp: vs_all_heap_simps obj_at_kh_kheap_simps is_sc_obj_def)
-  apply simp
-  done
-
-lemma valid_tcb_state'_sc_update:
-  "\<lbrakk> valid_objs' s; valid_sched_context' sc' s; sc_at' scPtr s;  ksPSpace s x = Some (KOTCB obj) \<rbrakk>
-     \<Longrightarrow> valid_tcb_state' (tcbState obj) (s\<lparr>ksPSpace := ksPSpace s(scPtr \<mapsto> KOSchedContext sc')\<rparr>)"
-  apply (rule valid_objsE', simp, simp)
-  by (fastforce simp: typ_at'_same_type ps_clear_upd objBits_simps valid_obj'_def projectKOs
-                      valid_tcb_state'_def valid_bound_obj'_def valid_tcb'_def obj_at'_def
-               split: option.splits thread_state.splits)
-
-lemma valid_cap'_sc_update:
-  "\<lbrakk> valid_cap' cap s; valid_objs' s; valid_sched_context' sc' s; obj_at' (\<lambda>sc::sched_context. objBits sc = objBits sc') scPtr s \<rbrakk>
-     \<Longrightarrow> valid_cap' cap (s\<lparr>ksPSpace := ksPSpace s(scPtr \<mapsto> KOSchedContext sc')\<rparr>)"
-  supply ps_clear_upd[simp]
-  apply (clarsimp simp: typ_at'_same_type ko_wp_at'_def cte_at'_same_type
-                        valid_cap'_def obj_at'_def projectKOs objBits_simps
-                 split: capability.splits)
-         apply fastforce+
-       apply (clarsimp split: zombie_type.splits simp: projectKOs obj_at'_def typ_at'_same_type)
-       apply (intro conjI impI; clarsimp)
-        apply (drule_tac x=addr in spec, clarsimp)
-       apply (drule_tac x=addr in spec, clarsimp)
-      apply (clarsimp simp: ko_wp_at'_def valid_cap'_def obj_at'_def projectKOs objBits_simps
-                            page_directory_at'_def page_table_at'_def scBits_simps
-                     split: ARM_H.arch_capability.splits option.splits if_split_asm
-           | rule_tac ko="KOSchedContext obj" in typ_at'_same_type[where p'=scPtr]
-           | simp)+
-     apply fastforce
-    apply (clarsimp simp: valid_untyped'_def ko_wp_at'_def obj_range'_def split: if_split_asm)
-     apply (drule_tac x=scPtr in spec, fastforce simp: objBits_simps)+
-   apply (drule_tac x=addr in spec, fastforce)
-  apply fastforce
+    apply (rule corres_split[OF updateRefillHd_corres], simp)
+       apply (clarsimp simp: refill_map_def)
+      apply (rule updateRefillTl_corres, simp)
+      apply (clarsimp simp: refill_map_def)
+     apply (wpsimp simp: update_refill_hd_rewrite wp: set_refills_wp get_refills_wp)
+    apply (wpsimp wp: hoare_vcg_conj_lift)
+     apply (wpsimp simp: updateRefillHd_def wp: updateSchedContext_wp)
+    apply (wpsimp wp: updateRefillHd_valid_objs')
+   apply (clarsimp simp: obj_at_def is_active_sc2_def is_sc_obj
+                  split: option.split_asm Structures_A.kernel_object.split_asm)
+  apply (clarsimp simp: obj_at_simps fun_upd_def[symmetric] scBits_simps ps_clear_upd)
+  apply (erule (1) valid_objsE')
+  apply (clarsimp simp: is_active_sc'_def valid_obj'_def valid_sched_context'_def
+                 split: option.split_asm)
   done
 
 lemmas sc_relation_refillResetRR1 =
   sc_relation_updateRefillTl[where f="r_amount_update (\<lambda>_. 0)" and f'="rAmount_update (\<lambda>_. 0)"]
-
-lemma take_drop_nth:
-  "\<lbrakk> 0 < n; n < length ls\<rbrakk> \<Longrightarrow> take 1 (drop n ls) = [ls ! n]"
-  apply (induct ls arbitrary: n; clarsimp simp: drop_Cons nth_Cons)
-  by (case_tac n; simp add: drop_Suc_nth)
 
 lemma sc_relation_refillResetRR2:
   "\<lbrakk>sc_relation sc n sc'; length (sc_refills sc) = 2; sc_refill_max sc = MIN_REFILLS;
@@ -976,52 +1025,39 @@ lemma sc_relation_refillResetRR:
   apply (drule sc_relation_refillResetRR2; fastforce?)
   by (drule sc_relation_refillResetRR1; clarsimp simp: refill_map_def)
 
-lemma length_refills_map[simp]:
-  "\<lbrakk> mx \<le> length list; count \<le> mx \<rbrakk> \<Longrightarrow> length (refills_map start count mx list) = count"
-  by (clarsimp simp: refills_map_def)
-
 lemma refillResetRR_corres:
-  "corres dc (pspace_aligned and pspace_distinct and sc_at csc_ptr and is_active_sc csc_ptr
+  "corres dc (sc_at csc_ptr and is_active_sc csc_ptr
                   and round_robin csc_ptr and valid_refills csc_ptr)
-             valid_objs'
+             (valid_objs' and sc_at' csc_ptr)
              (refill_reset_rr csc_ptr) (refillResetRR csc_ptr)"
   (is "corres dc ?abs ?conc _ _")
-  apply (rule_tac Q="active_sc_at' csc_ptr" in corres_cross_add_guard)
-   apply (simp add: active_sc_at_equiv[symmetric])
-   apply (fastforce elim: active_sc_at_cross[OF state_relation_pspace_relation])
-  apply (rule_tac Q="obj_at' (\<lambda>sc'. length (refills_map (scRefillHead sc') (scRefillCount sc')
-                                                    (scRefillMax sc') (scRefills sc')) = 2) csc_ptr"
+  supply projection_rewrites[simp]
+  apply (subst is_active_sc_rewrite)
+  apply (subst valid_refills_rewrite)
+  apply (rule_tac Q="is_active_sc' csc_ptr" in corres_cross_add_guard)
+   apply (fastforce dest!: is_active_sc'_cross[OF state_relation_pspace_relation])
+  apply (rule_tac Q="\<lambda>s'. ((\<lambda>sc'. scRefillCount sc' = 2) |< scs_of' s') csc_ptr"
          in corres_cross_add_guard)
-   apply (clarsimp simp: active_sc_at'_def valid_refills_def rr_valid_refills_def vs_all_heap_simps
-                         round_robin_def obj_at'_def projectKOs obj_relation_cuts_def
-                  dest!: pspace_relation_absD[where x=csc_ptr, OF _ state_relation_pspace_relation])
+   apply (clarsimp simp: obj_at'_def projectKOs round_robin2_def obj_at_def is_sc_obj
+                         rr_valid_refills_def is_active_sc2_def is_active_sc'_def)
    apply (drule (1) pspace_relation_absD[where x=csc_ptr, OF _ state_relation_pspace_relation])
-   apply (clarsimp simp: sc_relation_def opt_map_left_Some MIN_REFILLS_def split: if_split_asm)
-
-  apply (clarsimp simp: sc_at_pred_n_def obj_at_def is_sc_obj_def)
+   apply (erule (1) valid_objsE')
+   apply (clarsimp simp: sc_relation_def refills_map_def valid_sched_context'_def valid_obj'_def)
   apply (clarsimp simp: refill_reset_rr_def refillResetRR_def get_refills_def updateRefillTl_def
                         update_sched_context_decompose[symmetric, simplified] update_refill_tl_def)
   apply (rule corres_guard_imp)
     apply (rule monadic_rewrite_corres'[OF _ monadic_rewrite_sym[OF updateSchedContext_decompose[simplified]]])
-    apply (rule updateSchedContext_corres_gen[where
-                P="\<lambda>sc. length (sc_refills sc) = 2 \<and> sc_refill_max sc = MIN_REFILLS"
-            and P'="\<lambda>sc'. scRefillMax sc' \<le> length (scRefills sc')
-                        \<and> scRefillHead sc' < scRefillMax sc'
-                        \<and> scRefillCount sc' \<le> scRefillMax sc' \<and> 1 < scRefillCount sc'"])
-      apply (intro allI impI)
-      apply (rule sc_relation_refillResetRR; simp)
-     apply clarsimp
-    apply (clarsimp simp: objBits_simps)
-   apply (clarsimp simp: vs_all_heap_simps obj_at_def is_sc_obj sc_of_def opt_map_def
-                         round_robin_def valid_refills_def rr_valid_refills_def)
-  apply (clarsimp simp: active_sc_at'_def)
-  apply (drule obj_at_ko_at', clarsimp)
-  apply (frule (1) sc_ko_at_valid_objs_valid_sc')
-  by (clarsimp simp: obj_at'_def projectKOs opt_map_left_Some valid_sched_context'_def objBits_simps)
-
-lemma wrap_slice_start_0:
-  "\<lbrakk>0 < count; mx \<le> length ls; count \<le> mx\<rbrakk> \<Longrightarrow> wrap_slice 0 count mx ls = take count ls"
-  by (clarsimp simp: wrap_slice_def)
+    apply (rule updateSchedContext_corres_gen'[where
+                 P="(\<lambda>s. ((\<lambda>sc. length (sc_refills sc) = 2 \<and> sc_refill_max sc = MIN_REFILLS) |< scs_of2 s) csc_ptr)"
+            and P'="valid_objs' and is_active_sc' csc_ptr and (\<lambda>s'. ((\<lambda>sc'. scRefillCount sc' = 2) |< scs_of' s') csc_ptr)"])
+      apply (clarsimp, drule (3) state_relation_sc_relation)
+      apply (clarsimp simp: is_sc_obj obj_at_simps is_active_sc'_def)
+      apply (erule (1) valid_objsE', clarsimp simp: valid_obj'_def valid_sched_context'_def)
+      apply (fastforce elim!: sc_relation_refillResetRR[simplified])
+     apply (fastforce simp: obj_at_simps is_sc_obj dest!: state_relation_sc_replies_relation_sc)
+     apply (clarsimp simp: objBits_simps)+
+   apply (clarsimp simp: round_robin2_def obj_at_def is_sc_obj rr_valid_refills_def)
+  by (clarsimp simp: objBits_simps)
 
 lemma refillPopHead_corres:
   "corres (\<lambda>refill refill'. refill = refill_map refill')
@@ -1031,67 +1067,42 @@ lemma refillPopHead_corres:
               (refill_pop_head sc_ptr) (refillPopHead sc_ptr)"
   (is "corres _ ?abs ?conc _ _")
   supply if_split[split del]
+  supply projection_rewrites[simp]
+  apply (subst is_active_sc_rewrite)
   apply (rule corres_cross[where Q' = "sc_at' sc_ptr", OF sc_at'_cross_rel], fastforce)
+  apply (rule_tac Q="is_active_sc' sc_ptr" in corres_cross_add_guard)
+   apply (fastforce dest!: is_active_sc'_cross[OF state_relation_pspace_relation])
   apply (clarsimp simp: refill_pop_head_def refillPopHead_def)
   apply (clarsimp simp: getRefillNext_getSchedContext get_refills_def liftM_def)
   apply (rule corres_split'[rotated 2, OF get_sched_context_sp get_sc_sp'])
    apply (rule corres_guard_imp)
      apply (rule get_sc_corres)
     apply simp
-   apply (clarsimp simp: active_sc_at'_def elim: obj_at'_weakenE)
+   apply simp
   apply (rename_tac sc')
-  apply (rule_tac F="scRefillMax sc' \<le> length (scRefills sc') \<and> (scRefillHead sc' < scRefillMax sc'
-                     \<and> scRefillCount sc' \<le> scRefillMax sc' \<and> 0 < scRefillCount sc')" in corres_req)
-   apply clarsimp
-   apply (drule sc_ko_at_valid_objs_valid_sc'; clarsimp simp: valid_sched_context'_def)
-   apply (clarsimp simp: projectKOs active_sc_at'_def obj_at'_def sc_relation_def vs_all_heap_simps
-                         active_sc_def obj_at_def)
+  apply (rule_tac F="refill_hd sc = refill_map (refillHd sc')" in corres_req)
+   apply (clarsimp simp: obj_at_def is_sc_obj obj_at'_def projectKOs)
+   apply (frule (1) pspace_relation_absD[OF _ state_relation_pspace_relation])
+   apply (clarsimp elim!: refill_hd_relation)
+   apply (erule (1) valid_objsE', clarsimp simp: valid_obj'_def valid_sched_context'_def is_active_sc'_def)
   apply (rule corres_guard_imp)
-    apply (rule corres_split'[OF updateSchedContext_corres_gen[where
-                                    P="\<lambda>sc. 1 < length (sc_refills sc)"
-                                and P'="\<lambda>sc'. scRefillMax sc' \<le> length (scRefills sc')
-                                              \<and> (scRefillHead sc' < scRefillMax sc'
-                                              \<and> scRefillCount sc' \<le> scRefillMax sc'
-                                              \<and> 0 < scRefillCount sc')"]])
-         apply (clarsimp simp: sc_relation_def refills_map_def tl_map)
+    apply (rule corres_split'[OF updateSchedContext_corres_gen'[where
+                                    P="(\<lambda>s. ((\<lambda>sc. 1 < length (sc_refills sc)) |< scs_of2 s) sc_ptr)"
+                                and P'="valid_objs' and is_active_sc' sc_ptr"]])
+         apply (clarsimp, drule (3) state_relation_sc_relation)
+         apply (clarsimp simp: sc_relation_def refills_map_def tl_map obj_at_simps is_sc_obj)
+         apply (erule (1) valid_objsE', clarsimp simp: valid_obj'_def valid_sched_context'_def)
          apply (subst tl_wrap_slice; clarsimp simp: min_def split: if_split)
          apply (rule conjI impI; clarsimp simp: refillNextIndex_def wrap_slice_start_0 split: if_splits)
+        apply (fastforce simp: obj_at_simps is_sc_obj dest!: state_relation_sc_replies_relation_sc)
         apply clarsimp
        apply (clarsimp simp: objBits_simps)
       apply simp
-      apply (prop_tac "refills_map (scRefillHead sc') (scRefillCount sc')
-                       (scRefillMax sc') (scRefills sc') \<noteq> []")
-       apply (clarsimp intro!: neq_Nil_lengthI simp: refills_map_def)
-      apply (clarsimp simp: sc_relation_def refills_map_def hd_map refillHd_def hd_wrap_slice)
      apply (wpsimp wp: update_sched_context_wp)
     apply (wpsimp wp: updateSchedContext_wp)
-   apply (clarsimp simp: sc_refills_sc_at_def obj_at_def sc_of_def opt_map_def)
-  apply (clarsimp simp: obj_at'_def projectKOs opt_map_left_Some)
+   apply (clarsimp simp: sc_refills_sc_at_def obj_at_def)
+  apply simp
   done
-
-lemma updateSchedContext_decompose_twice:
-  "\<lbrakk>\<forall>sc. objBits (f sc) = objBits sc; \<forall>sc. objBits (g sc) = objBits sc;
-     \<forall>sc. objBits (h sc) = objBits sc\<rbrakk> \<Longrightarrow>
-    monadic_rewrite False True
-     (sc_at' scPtr)
-     (updateSchedContext scPtr (h o g o f))
-     (do updateSchedContext scPtr f;
-         updateSchedContext scPtr g;
-         updateSchedContext scPtr h
-      od)"
-  apply (rule monadic_rewrite_imp)
-   apply (rule monadic_rewrite_trans)
-    apply (rule updateSchedContext_decompose)
-   apply (rule monadic_rewrite_bind_tail)
-    apply simp
-    apply (rule updateSchedContext_decompose[simplified])
-   apply (wpsimp wp: updateSchedContext_wp)
-  apply (clarsimp simp: obj_at'_def projectKOs ps_clear_upd objBits_def)
-  done
-
-abbreviation
-  opt_pred :: "('a \<Rightarrow> bool) \<Rightarrow> 'a option \<Rightarrow> bool" (infixl "|P" 50) where
-  "P |P opt \<equiv> case_option False P opt"
 
 lemma refillNew_corres:
   "\<lbrakk>1 < max_refills; valid_refills_number' max_refills (min_sched_context_bits + n)\<rbrakk>
@@ -1099,369 +1110,242 @@ lemma refillNew_corres:
          (pspace_aligned and pspace_distinct and sc_obj_at n sc_ptr) \<top>
             (refill_new sc_ptr max_refills budget period)
             (refillNew sc_ptr max_refills budget period)"
+  supply projection_rewrites[simp]
+  supply getSchedContext_wp[wp del] set_sc'.get_wp[wp del]
   apply (rule corres_cross_add_guard[where
-      Q = "sc_at' sc_ptr and (\<lambda>s'. (\<lambda>sc. objBits sc = minSchedContextBits + n) |P scs_of' s' sc_ptr)"])
+      Q = "sc_at' sc_ptr and (\<lambda>s'. ((\<lambda>sc. objBits sc = minSchedContextBits + n) |< scs_of' s') sc_ptr)"])
    apply (fastforce dest!: sc_obj_at_cross[OF state_relation_pspace_relation]
-                     simp: obj_at'_def pred_map_simps projectKOs opt_map_def)
+                     simp: obj_at'_def projectKOs)
   apply (unfold refillNew_def refill_new_def setRefillHd_def updateRefillHd_def)
-  apply (rule corres_split'[OF _ _ gets_sp getCurTime_sp])
-   apply (rule corres_guard_imp)
-     apply (rule getCurTime_corres)
-    apply simp+
-  apply (rule stronger_corres_guard_imp)
-    (* period *)
-    apply (rule corres_split[OF updateSchedContext_corres]; (clarsimp simp: sc_relation_def objBits_simps)?)
-      (* budget *)
-      apply (rule corres_split[OF updateSchedContext_corres]; (clarsimp simp: sc_relation_def objBits_simps)?)
-        (* max_refills, sc_refills update *)
-        (* rewrite into one step updateSchedContext corres *)
-        apply (subst bind_assoc[symmetric])
-        apply (subst update_sched_context_decompose[symmetric, simplified])
-        apply (subst bind_assoc[symmetric])
-        apply (subst bind_assoc[symmetric])
-        apply (subst bind_assoc)
-        apply (rule corres_split[OF  monadic_rewrite_corres'
-                                       [OF _ monadic_rewrite_sym
-                                               [OF updateSchedContext_decompose_twice[simplified]]]])
-              (* use setSchedContext_corres *)
-              apply (rule monadic_rewrite_corres[OF _ update_sched_context_rewrite[where n=n]])
-              apply (simp add: updateSchedContext_def)
-              apply (rule corres_split[OF get_sc_corres])
-                apply (rename_tac sc')
-                apply (rule_tac P="ko_at (kernel_object.SchedContext sc n) sc_ptr"
-                            and P'="ko_at' sc' sc_ptr
-                                    and (\<lambda>s'. (\<lambda>sc. objBits sc = minSchedContextBits + n) |P scs_of' s' sc_ptr)"
-                       in corres_inst)
-                apply (rule_tac F="length (scRefills sc') = max_num_refills (min_sched_context_bits + n)"
-                       in corres_req)
-                 apply (clarsimp simp: obj_at'_def projectKOs opt_map_left_Some objBits_simps scBits_simps)
-                using scBits_inverse_sc apply fastforce
-                apply (rule stronger_corres_guard_imp)
-                  apply (rule_tac sc'="sc'\<lparr> scRefillMax := max_refills,
-                                            scRefillHead := 0,
-                                            scRefillCount := Suc 0,
-                                            scRefills := updateAt 0 (scRefills sc') (\<lambda>r. Refill curTime budget)\<rparr>"
-                         in setSchedContext_corres)
-                   apply (clarsimp simp: sc_relation_def refill_map_def refills_map_def
-                                         wrap_slice_start_0 valid_refills_number'_def
-                                         max_num_refills_eq_refillAbsoluteMax')
-                   apply (case_tac "scRefills sc'"; simp add: updateAt_def null_def refill_map_def)
-                  apply (clarsimp simp: objBits_simps scBits_simps)
-                 apply simp
-                apply (clarsimp simp: objBits_simps scBits_simps obj_at'_def projectKOs obj_at_def is_sc_obj
-                               dest!: state_relation_sc_replies_relation)
-                apply (fastforce elim!: sc_replies_relation_prevs_list)
-               apply wpsimp+
-             apply (clarsimp simp: objBits_simps)+
-          (* last step : add tail *)
-          apply (rule maybeAddEmptyTail_corres[simplified dc_def])
+  apply (rule corres_guard_imp)
+    apply (rule corres_split_eqr[OF _ getCurTime_corres])
+      (* period *)
+      apply (rule corres_split[OF updateSchedContext_corres]; clarsimp simp: objBits_simps)
+     apply (fastforce simp: obj_at_simps is_sc_obj sc_relation_def
+                     dest!: state_relation_sc_relation)
+     apply (fastforce simp: obj_at_simps is_sc_obj dest!: state_relation_sc_replies_relation_sc)
+        (* budget *)
+        apply (rule corres_split[OF updateSchedContext_corres]; (clarsimp simp: objBits_simps)?)
+     apply (fastforce simp: obj_at_simps is_sc_obj sc_relation_def
+                     dest!: state_relation_sc_relation)
+           apply (fastforce simp: obj_at_simps is_sc_obj dest!: state_relation_sc_replies_relation_sc)
+          (* max_refills, sc_refills update *)
+          (* rewrite into one step updateSchedContext corres *)
+          apply (rename_tac ctime)
+          apply (rule_tac P="sc_obj_at n sc_ptr and (\<lambda>s. ctime = cur_time s)"
+                      and P'="sc_at' sc_ptr and (\<lambda>s'. ctime = ksCurTime s')
+                              and (\<lambda>s'. ((\<lambda>sc'. objBits sc' = minSchedContextBits + n) |< scs_of' s') sc_ptr)"
+                 in corres_inst)
+          apply (subst bind_assoc[symmetric])
+          apply (subst update_sched_context_decompose[symmetric, simplified])
+          apply (subst bind_assoc[symmetric])
+          apply (subst bind_assoc[symmetric])
+          apply (subst bind_assoc)
+          apply (rule corres_guard_imp)
+            apply (rule corres_split[OF  monadic_rewrite_corres'
+                                           [OF _ monadic_rewrite_sym
+                                                   [OF updateSchedContext_decompose_twice[simplified]]]])
+                  (* use setSchedContext_corres *)
+                  apply (rule monadic_rewrite_corres[OF _ update_sched_context_rewrite[where n=n]])
+                  apply (simp add: updateSchedContext_def)
+                  apply (rule corres_split[OF get_sc_corres])
+                    apply (rename_tac sc')
+                    apply (rule_tac P="ko_at (kernel_object.SchedContext sc n) sc_ptr"
+                                and P'="ko_at' sc' sc_ptr
+                                        and (\<lambda>s'. ((\<lambda>sc'. objBits sc' = minSchedContextBits + n) |< scs_of' s') sc_ptr)"
+                           in corres_inst)
+                    apply (rule_tac F="length (scRefills sc') = max_num_refills (min_sched_context_bits + n)"
+                           in corres_req)
+                     apply (clarsimp simp: obj_at'_def projectKOs objBits_simps scBits_simps)
+                    using scBits_inverse_sc apply fastforce
+                    apply (rule stronger_corres_guard_imp)
+                      apply (rule_tac sc'="sc'\<lparr> scRefillMax := max_refills,
+                                                scRefillHead := 0,
+                                                scRefillCount := Suc 0,
+                                                scRefills := updateAt 0 (scRefills sc') (\<lambda>r. Refill ctime budget)\<rparr>"
+                             in setSchedContext_corres)
+                       apply (clarsimp simp: sc_relation_def refills_map_def valid_refills_number'_def
+                                             wrap_slice_start_0 max_num_refills_eq_refillAbsoluteMax')
+                       apply (case_tac "scRefills sc'"; simp add: updateAt_def null_def refill_map_def)
+                      apply (clarsimp simp: objBits_simps scBits_simps)
+                     apply simp
+                    apply (fastforce simp: obj_at_simps is_sc_obj
+                                    dest!: sc_replies_relation_prevs_list'[OF state_relation_sc_replies_relation])
+                   apply (wpsimp wp: getSchedContext_wp')+
+                 apply (clarsimp simp: objBits_simps)+
+              (* last step : add tail *)
+              apply (rule_tac P="sc_obj_at n sc_ptr and is_active_sc2 sc_ptr"
+                          and P'="sc_at' sc_ptr
+                                  and (\<lambda>s'. ((\<lambda>sc'. objBits sc' = minSchedContextBits + n
+                                             \<and> scRefillHead sc' = 0 \<and> scRefillCount sc' = 1
+                                             \<and> scRefillMax sc' = max_refills) |< scs_of' s') sc_ptr)"
+                     in corres_inst)
+              apply (rule stronger_corres_guard_imp)
+                apply (rule maybeAddEmptyTail_corres[simplified dc_def])
+               apply simp
+              apply (clarsimp simp: obj_at_simps is_sc_obj objBits_simps scBits_simps
+                                    valid_refills_number'_def)
+              apply (drule (1) pspace_relation_absD[OF _ state_relation_pspace_relation, rotated])
+              using scBits_inverse_sc apply fastforce
+             apply (wpsimp wp: update_sched_context_wp updateSchedContext_wp)+
+           apply (clarsimp simp:  obj_at_def is_sc_obj is_active_sc2_def)
+          apply (clarsimp simp: obj_at_simps fun_upd_def[symmetric] valid_objs'_def ps_clear_upd)
          apply (wpsimp wp: update_sched_context_wp updateSchedContext_wp)+
-   apply (clarsimp simp: vs_all_heap_simps obj_at_def is_sc_obj active_sc_def sc_of_def)
-  apply (clarsimp simp: obj_at'_def projectKOs ps_clear_upd objBits_simps scBits_simps obj_at_def
-                        opt_map_left_Some fun_upd_def[symmetric] valid_refills_number'_def is_sc_obj)
-  apply (drule (1) pspace_relation_absD[OF _ state_relation_pspace_relation])
-  apply (clarsimp dest!: scBits_inverse_sc simp: updateAt_def null_def)
+   apply (clarsimp simp:  obj_at_def is_sc_obj is_active_sc2_def)
+  apply (clarsimp simp: obj_at_simps fun_upd_def[symmetric] valid_objs'_def ps_clear_upd)
   done
 
-lemma refill_update_bundled:
-  "refill_update sc_ptr period budget max_refills
-   = (do sc \<leftarrow> get_sched_context sc_ptr;
-         head \<leftarrow> return (refill_hd sc);
-         update_sched_context sc_ptr (\<lambda>sc. sc\<lparr>sc_refill_max := max_refills,
-                                              sc_refills := [head]\<rparr>);
-         set_sc_obj_ref sc_period_update sc_ptr period;
-         set_sc_obj_ref sc_budget_update sc_ptr budget;
-         ready \<leftarrow> get_sc_refill_ready sc_ptr;
-         when ready $ do cur_time \<leftarrow> gets cur_time;
-                         update_refill_hd sc_ptr (r_time_update (\<lambda>_. cur_time))
-                      od;
-         sc \<leftarrow> get_sched_context sc_ptr;
-         refill_hd \<leftarrow> return (refill_hd sc);
-         if budget \<le> r_amount refill_hd
-            then do update_refill_hd sc_ptr (r_amount_update (\<lambda>_. budget));
-                    maybe_add_empty_tail sc_ptr
-                 od
-            else do unused \<leftarrow> return $ budget - r_amount refill_hd;
-                    new \<leftarrow> return \<lparr>r_time = r_time refill_hd + period, r_amount = unused\<rparr>;
-                    refill_add_tail sc_ptr new
-                 od
-      od)"
-  apply (rule monadic_rewrite_to_eq)
-  apply (clarsimp simp: refill_update_def)
-  apply (simp flip: bind_assoc)
-  apply (rule monadic_rewrite_bind_head)+
-  apply (rule monadic_rewrite_bind_tail)
-  apply (clarsimp simp: monadic_rewrite_def set_refills_def)
-  apply (simp add: update_sched_context_decompose_ext2
-                       [where f=sc_refills_update and g=sc_refill_max_update]
-                   bind_assoc)
-  apply wpsimp
-  oops
-
-lemma refillUpdate_bundled:
-  "monadic_rewrite False True (sc_at' scPtr)
-     (refillUpdate scPtr newPeriod newBudget newMaxRefills)
-     (do sc \<leftarrow> getSchedContext scPtr;
-         do sca \<leftarrow> getSchedContext scPtr;
-            setSchedContext scPtr
-             (scRefills_update (\<lambda>_. replaceAt 0 (scRefills sca) (refillHd sc))
-              (scRefillMax_update (\<lambda>_. newMaxRefills)
-               (scRefillCount_update (\<lambda>_. 1)
-                (scRefillHead_update (\<lambda>_. 0) sca))))
-         od;
-         sc \<leftarrow> getSchedContext scPtr;
-         setSchedContext scPtr (scPeriod_update (\<lambda>_. newPeriod) sc);
-         sc \<leftarrow> getSchedContext scPtr;
-         setSchedContext scPtr (scBudget_update (\<lambda>_. newBudget) sc);
-         whenM (refillReady scPtr) $ do curTime \<leftarrow> getCurTime;
-                                        updateRefillHd scPtr (rTime_update (\<lambda>_. curTime))
-                                     od;
-         head \<leftarrow> liftM refillHd $ getSchedContext scPtr;
-         if newBudget \<le> rAmount head then do updateRefillHd scPtr (rAmount_update (\<lambda>_. newBudget));
-                                             maybeAddEmptyTail scPtr
-                                          od
-         else do unused \<leftarrow> return (newBudget - rAmount head);
-                 new \<leftarrow> return ( Refill_ \<lparr> rTime= rTime head + newPeriod, rAmount= unused \<rparr>);
-                 refillAddTail scPtr new
-        od
-      od)"
-  apply (clarsimp simp: refillUpdate_def setRefillIndex_def)
-  apply (simp flip: bind_assoc)
-  apply (rule monadic_rewrite_bind_head)+
-  apply (simp add: bind_assoc)
-  apply (rule monadic_rewrite_bind_tail[rotated, OF get_sc_inv'])
-  apply (subst bind_assoc_group4)
-  apply (rule monadic_rewrite_rewrite_head)
-   apply (rule monadic_rewrite_imp)
-    apply (rule monadic_rewrite_sym)
-    apply (rule getSchedContext_setSchedContext_decompose_decompose_ext2[unfolded K_bind_def])
-   apply (clarsimp simp: objBits_simps)
-  apply (simp only: bind_assoc)
-  apply (subst bind_assoc_group4)
-  apply (rule monadic_rewrite_rewrite_head)
-   apply (rule monadic_rewrite_imp)
-    apply (rule monadic_rewrite_sym)
-    apply (rule getSchedContext_setSchedContext_decompose_decompose_ext2[unfolded K_bind_def])
-   apply (clarsimp simp: objBits_simps)
-  apply (simp only: bind_assoc)
-  apply (rule monadic_rewrite_imp)
-   apply (rule monadic_rewrite_trans_dup)
-    apply (rule monadic_rewrite_sym)
-    apply (rule getSchedContext_setSchedContext_decompose[unfolded K_bind_def])
-   apply (rule monadic_rewrite_refl3)
-   apply clarsimp
-  apply (fastforce simp: objBits_simps length_replaceAt)
-  oops
-
 lemma refillUpdate_corres:
-  "1 < max_refills
+  "\<lbrakk>1 < max_refills; valid_refills_number' max_refills (min_sched_context_bits + n)\<rbrakk>
    \<Longrightarrow> corres dc
-              ((valid_objs and pspace_aligned and pspace_distinct and is_active_sc sc_ptr
-                and sc_at sc_ptr) and active_sc_valid_refills)
-              (\<lambda>s'. \<exists>n. sc_at'_n n sc_ptr s' \<and> valid_refills_number' max_refills n \<and> valid_objs' s')
-              (refill_update sc_ptr period budget max_refills )
+              ((is_active_sc2 sc_ptr and sc_obj_at n sc_ptr) and (pspace_aligned and pspace_distinct))
+              (\<lambda>s'. ((\<lambda>sc'. std_sc' sc') |< scs_of' s') sc_ptr)
+              (refill_update sc_ptr period budget max_refills)
               (refillUpdate sc_ptr period budget max_refills)"
-  (is "_ \<Longrightarrow> corres _ (?pred and _) ?conc _ _")
-  apply (rule corres_cross[where Q' = "sc_at' sc_ptr", OF sc_at'_cross_rel], fastforce)
-  apply (rule_tac Q="active_sc_at' sc_ptr" in corres_cross_add_guard)
-   apply (rule active_sc_at'_cross, simp+)
-
-
-
-
-
-
-
-
-  apply (subst refill_update_bundled)
-  apply (rule monadic_rewrite_corres'
-               [where P'=P' and Q=P' for P', simplified pred_conj_def, simplified, rotated])
-   apply (rule monadic_rewrite_imp)
-    apply (rule refillUpdate_bundled)
-apply (fold updateSchedContext_def)+
-   apply simp
-
-  apply (rule corres_split'[rotated 2, OF get_sched_context_sp get_sc_sp'])
-   apply (corressimp corres: get_sc_corres)
-  apply (rename_tac sc')
-  apply clarsimp
-  apply (subst update_sched_context_def)
-  apply (clarsimp simp: bind_assoc)
-  apply (rule corres_symb_exec_r[OF _ get_sc_sp', rotated]; (solves wpsimp)?)
-  apply (rename_tac sc'')
-  apply (rule_tac F="sc'' = sc'" in corres_req)
-   apply (clarsimp simp: obj_at'_def)
-  apply (clarsimp simp: pred_conj_def cong: conj_cong)
-  apply (rule corres_symb_exec_l[OF _ _ get_object_sp, rotated]; (solves wpsimp)?)
-    apply (fastforce intro: get_object_exs_valid simp: obj_at_def)
-   apply (wpsimp simp: obj_at_def)
-  apply (rename_tac obj)
-  apply (case_tac obj
-         ; clarsimp; (solves \<open>corressimp corres: corres_False simp: obj_at_def is_sc_obj_def\<close>)?)
-  apply (rename_tac abs_sc abs_n)
-  apply (rule_tac F="abs_sc = sc" in corres_req)
-   apply (clarsimp simp: obj_at_def)
-  apply clarsimp
-  apply (rule_tac Q="sc_obj_at (objBits sc' - minSchedContextBits) sc_ptr"
-               in corres_cross_add_abs_guard)
-   apply (fastforce dest!: state_relationD ko_at'_cross)
-
-  apply (rule_tac Q="\<lambda>_. ?pred and sc_refills_sc_at (\<lambda>refills. length refills = 1) sc_ptr"
-              and Q'="\<lambda>_. ?conc and sc_at' sc_ptr
-                          and obj_at' (\<lambda>sc. scRefillHead sc = 0 \<and> scRefillCount sc = 1
-                                            \<and> scRefillMax sc = max_refills) sc_ptr"
-               in corres_split'[rotated 2])
-     apply ((wpsimp wp: update_sched_context_valid_objs_update | wpsimp wp: set_object_wp)+)[1]
-     apply (fastforce dest!: active_sc_valid_refillsE
-                       simp: valid_refills_def vs_all_heap_simps rr_valid_refills_def
-                             valid_obj_def valid_sched_context_def active_sc_def sc_at_pred_n_def
-                             obj_at_def is_sc_obj_def)
-    apply ((wpsimp wp: hoare_vcg_ex_lift hoare_vcg_conj_lift | wpsimp wp: set_sc'.set_wp)+)[1]
-    apply (frule (1) sc_ko_at_valid_objs_valid_sc')
-    apply (fastforce simp: valid_sched_context'_def length_replaceAt valid_refills_number'_def
-                           obj_at'_def projectKOs objBits_simps' ko_wp_at'_def scBits_inverse_sc
-                           valid_sched_context_size'_def)
-
-   apply (rule corres_assume_pre)
-   apply (rule corres_guard_imp)
-     apply (rule_tac f="\<lambda>sc. sc\<lparr>sc_refill_max := max_refills, sc_refills := [refill_hd sc]\<rparr>"
-                 and f'="\<lambda>sc'. scRefills_update (\<lambda>_. replaceAt 0 (scRefills sc') (refillHd sc'))
-                                (scRefillMax_update (\<lambda>_. max_refills)
-                                 (scRefillCount_update (\<lambda>_. Suc 0)
-                                  (scRefillHead_update (\<lambda>_. 0) sc')))"
-                  in setSchedContext_no_stack_update_corres)
-        apply (clarsimp simp: sc_relation_def)
-        apply (prop_tac "max_refills \<le> length (replaceAt 0 (scRefills sc') (refillHd sc'))")
-         apply (clarsimp simp: valid_refills_number'_def obj_at'_def projectKOs objBitsKO_def
-                               ko_wp_at'_def scBits_simps length_replaceAt)
-        apply (prop_tac "0 < scRefillCount sc' \<and> scRefillHead sc' < scRefillMax sc'
-                         \<and> scRefillMax sc' \<le> length (scRefills sc') \<and> 0 < length (scRefills sc')")
-         apply (prop_tac "sc_relation sc n sc'")
-          apply (fastforce simp: sc_relation_def)
-         apply (frule (1) sc_ko_at_valid_objs_valid_sc')
-         apply (fastforce dest: sc_ko_at_valid_objs_valid_sc'
-                          simp: valid_sched_context'_def active_sc_at'_def obj_at'_def)
-        apply (intro conjI impI)
-         apply (clarsimp simp: refills_map_def)
-         apply (rule nth_equalityI; clarsimp)
-         apply (subst hd_conv_nth)
-          apply (rule length_greater_0_conv[THEN iffD1])
-          apply (subst length_map)
-          apply (subst length_wrap_slice; simp)
-         apply (subst nth_map)
-          apply (subst length_wrap_slice; simp)
-         apply (subst wrap_slice_index; simp)+
-         apply (subst replaceAt_index; fastforce simp: refillHd_def)
-        apply (fastforce simp: length_replaceAt)
-       apply fastforce
-      apply (fastforce simp: length_replaceAt objBits_simps)
-     apply simp
-    apply (clarsimp simp: obj_at_def)
-   apply (clarsimp simp: obj_at'_def)
-
-  apply (rule corres_symb_exec_r[OF _ get_sc_sp', rotated]; (solves wpsimp)?)
-  apply (rule_tac Q="\<lambda>_. ?pred and sc_refills_sc_at (\<lambda>refills. length refills = 1) sc_ptr"
-              and Q'="\<lambda>_. ?conc and sc_at' sc_ptr
-                          and obj_at' (\<lambda>sc. scRefillHead sc = 0 \<and> scRefillCount sc = 1
-                                            \<and> scRefillMax sc = max_refills) sc_ptr"
-               in corres_split'[rotated 2])
-     apply ((wpsimp wp: update_sched_context_valid_objs_update
-             | wpsimp wp: update_sched_context_wp)+)[1]
-     apply (fastforce dest!: valid_objs_ko_at
-                       simp: valid_obj_def valid_sched_context_def obj_at_def is_sc_obj_def
-                             sc_at_pred_n_def)
-    apply ((wpsimp wp: hoare_vcg_ex_lift hoare_vcg_conj_lift | wpsimp wp: set_sc'.set_wp)+)[1]
-    apply (frule (1) sc_ko_at_valid_objs_valid_sc')
-    apply (fastforce simp: valid_sched_context'_def length_replaceAt valid_refills_number'_def
-                           obj_at'_def projectKOs objBits_simps' valid_sched_context_size'_def
-                           ps_clear_def)
-   apply (corressimp corres: update_sc_no_reply_stack_update_ko_at'_corres
-                               [where f'="scPeriod_update (\<lambda>_. period)"]
-                       simp: sc_relation_def objBits_simps)
-
-  apply (rule corres_symb_exec_r[OF _ get_sc_sp', rotated]; (solves wpsimp)?)
-  apply (rule_tac Q="\<lambda>_. ?pred and sc_refills_sc_at (\<lambda>refills. length refills = 1) sc_ptr"
-              and Q'="\<lambda>_. ?conc and sc_at' sc_ptr
-                          and obj_at' (\<lambda>sc. scRefillHead sc = 0 \<and> scRefillCount sc = 1
-                                            \<and> scRefillMax sc = max_refills) sc_ptr"
-               in corres_split'[rotated 2])
-     apply ((wpsimp wp: update_sched_context_valid_objs_update
-             | wpsimp wp: update_sched_context_wp)+)[1]
-     apply (fastforce dest!: valid_objs_ko_at
-                       simp: valid_obj_def valid_sched_context_def obj_at_def is_sc_obj_def
-                             sc_at_pred_n_def)
-    apply ((wpsimp wp: hoare_vcg_ex_lift hoare_vcg_conj_lift | wpsimp wp: set_sc'.set_wp)+)[1]
-    apply (frule (1) sc_ko_at_valid_objs_valid_sc')
-    apply (fastforce simp: valid_sched_context'_def length_replaceAt valid_refills_number'_def
-                          obj_at'_def projectKOs objBits_simps' ko_wp_at'_def scBits_inverse_sc
-                          valid_sched_context_size'_def ps_clear_def)
-   apply (corressimp corres: update_sc_no_reply_stack_update_ko_at'_corres
-                               [where f'="scBudget_update (\<lambda>_. budget)"]
-                       simp: sc_relation_def objBits_simps)
-
-  apply (clarsimp simp: whenM_def ifM_def bind_assoc when_def getRefillNext_getSchedContext
-                        getRefillSize_def2 liftM_def)
-  apply (rule corres_split'[rotated 2, OF get_sc_refill_ready_inv refillReady_inv])
-   apply (corressimp corres: refillReady_corres)
-   apply (clarsimp simp: sc_at_pred_n_def obj_at_def)
-  apply (rule_tac Q="\<lambda>_. ?pred and sc_refills_sc_at (\<lambda>refills. length refills = 1) sc_ptr"
-              and Q'="\<lambda>_. valid_objs' and obj_at' (\<lambda>sc. scRefillHead sc = 0 \<and> scRefillCount sc = 1
-                                                         \<and> scRefillMax sc = max_refills) sc_ptr"
-              and r'=dc
-               in corres_split'[rotated 2])
-     apply (simp add: update_refill_hd_def set_refills_def)
-     apply ((wpsimp wp: update_sched_context_valid_objs_update get_refills_wp
-             | wpsimp wp: update_sched_context_wp get_refills_wp)+)[1]
-     apply (intro conjI impI allI)
-      apply (clarsimp simp: valid_sched_context_def)
-     apply (clarsimp simp: sc_at_pred_n_def obj_at_def)
-    apply ((wpsimp simp: updateRefillHd_def
-                     wp: set_sc'.valid_objs'
-            | wpsimp wp: set_sc'.set_wp)+)[1]
-    apply (fastforce dest: sc_ko_at_valid_objs_valid_sc'
-                     simp: valid_sched_context'_def valid_sched_context_size'_def objBits_simps
-                           valid_obj'_def length_replaceAt
-                           obj_at'_def projectKOs ps_clear_def)
-   apply (corressimp corres: getCurTime_corres updateRefillHd_corres
-                       simp: refill_map_def obj_at_kh_kheap_simps vs_all_heap_simps)
-   apply fastforce
-
-  apply clarsimp
-  apply (rule corres_split'[rotated 2, OF get_sched_context_sp get_sc_sp'])
-   apply (corressimp corres: get_sc_corres)
-  apply (rename_tac abs_sc conc_sc)
-  apply (rule_tac F="0 < scRefillCount conc_sc \<and> scRefillCount conc_sc \<le> scRefillMax conc_sc
-                     \<and> scRefillHead conc_sc < scRefillMax conc_sc
-                     \<and> scRefillMax conc_sc \<le> length (scRefills conc_sc)
-                     \<and> length (sc_refills abs_sc) = 1"
-               in corres_req)
-   apply (fastforce dest: sc_ko_at_valid_objs_valid_sc'
-                    simp: valid_sched_context'_def sc_relation_def sc_at_pred_n_def obj_at_def
-                          refills_map_def)
-  apply (clarsimp split del: if_split)
-  apply (frule_tac sc=abs_sc and sc'=conc_sc in refill_hd_relation; (solves simp)?)
-  apply (clarsimp simp: refill_map_def)
-  apply (intro conjI impI allI)
-   apply (rule corres_guard_imp)
-     apply (rule corres_split_deprecated[OF _ updateRefillHd_corres])
-         apply (rule maybeAddEmptyTail_corres)
-        apply simp
-       apply (clarsimp simp: refill_map_def)
-      apply (simp add: update_refill_hd_def set_refills_def)
-      apply ((wpsimp wp: update_sched_context_valid_objs_update get_refills_wp
-              | wpsimp wp: update_sched_context_wp get_refills_wp)+)[1]
-     apply (clarsimp simp: updateRefillHd_def)
-     apply (rule hoare_vcg_conj_lift
-            , (wpsimp wp: set_sc'.valid_objs'
-               | wpsimp wp: set_sc'.set_wp)+)[1]
-    apply (fastforce simp: obj_at_def active_sc_def vs_all_heap_simps sc_at_pred_n_def
-                           valid_sched_context_def)
-   apply (fastforce dest: sc_ko_at_valid_objs_valid_sc'
-                    simp: updateRefillHd_def valid_obj'_def valid_sched_context'_def
-                          valid_sched_context_size'_def length_replaceAt objBits_simps
-                          obj_at'_def projectKOs length_ineq_not_Nil(2))
-  apply (corressimp corres: refillAddTail_corres
-                      simp: obj_at'_def projectKOs refill_map_def obj_at_def is_sc_obj_def)
+  (is "_ \<Longrightarrow> _ \<Longrightarrow> corres _ (?pred and _) ?conc _ _")
+  supply getSchedContext_wp[wp del] set_sc'.get_wp[wp del] projection_rewrites[simp]
+  apply (rule corres_cross_add_guard[where
+      Q = "sc_at' sc_ptr and (\<lambda>s'. ((\<lambda>sc. objBits sc = minSchedContextBits + n) |< scs_of' s') sc_ptr)"])
+   apply (fastforce dest!: sc_obj_at_cross[OF state_relation_pspace_relation]
+                     simp: obj_at'_def projectKOs)
+  apply (rule_tac Q="is_active_sc' sc_ptr" in corres_cross_add_guard)
+   apply (rule is_active_sc'_cross, fastforce+)
+  apply (rule corres_guard_imp)
+    apply (rule_tac P="?pred" and P'="?conc and sc_at' sc_ptr" in corres_inst)
+    apply (unfold refillUpdate_def refill_update_def)
+    apply simp
+    (* rewrite the refill list update steps into one step updateSchedContext corres *)
+    apply (subst bind_assoc[where m="update_sched_context _ _", symmetric])
+    apply (subst update_sched_context_decompose[symmetric, simplified])
+    apply (subst bind_assoc[where m="updateSchedContext _ _", symmetric])
+    apply (subst bind_assoc[where m="do _ \<leftarrow> updateSchedContext _ _; updateSchedContext _ _ od", symmetric])
+    apply (subst bind_assoc[where m="do _ \<leftarrow> (do _ \<leftarrow> updateSchedContext _ _; updateSchedContext _ _ od);
+                                     updateSchedContext _ _ od", symmetric])
+    apply (subst bind_assoc[where m="updateSchedContext _ _"])
+    apply (subst bind_assoc[where m="updateSchedContext _ _"])
+    apply (subst bind_assoc[where m="updateSchedContext _ _"])
+    apply (rule stronger_corres_guard_imp)
+      apply (rule corres_split[OF  monadic_rewrite_corres'
+                                     [OF _ monadic_rewrite_sym
+                                             [OF updateSchedContext_decompose_thrice[simplified]]]])
+             (* now use setSchedContext_corres *)
+             apply (rule corres_inst[where P="?pred and sc_obj_at n sc_ptr" and P'="?conc and sc_at' sc_ptr"])
+             (* one of the sc_obj_at n sc_ptr will be consumed by the next line *)
+             apply (rule monadic_rewrite_corres[OF _ update_sched_context_rewrite[where n=n]])
+             apply (simp add: updateSchedContext_def)
+             apply (rule stronger_corres_guard_imp)
+               apply (rule corres_split[OF get_sc_corres])
+                 apply (rename_tac sc sc')
+                 apply (rule_tac P="?pred and ko_at (kernel_object.SchedContext sc n) sc_ptr"
+                             and P'="ko_at' sc' sc_ptr
+                                     and (\<lambda>s'. objBits sc' = minSchedContextBits + n
+                                                \<and> 0 < scRefillMax sc' \<and> std_sc' sc')"
+                        in corres_inst)
+                apply (rule_tac F="0 < scRefillMax sc' \<and> std_sc' sc'
+                                    \<and> length (scRefills sc') = max_num_refills (min_sched_context_bits + n)"
+                        in corres_req)
+                  apply clarsimp
+                  apply (clarsimp simp: obj_at'_def projectKOs objBits_simps scBits_simps)
+                  using scBits_inverse_sc apply fastforce
+                 apply (rule stronger_corres_guard_imp)
+                   apply (rule setSchedContext_corres)
+                    apply (unfold sc_relation_def; elim conjE exE; intro conjI; fastforce?)
+                    apply (clarsimp simp: refills_map_def wrap_slice_start_0 hd_map neq_Nil_lengthI
+                                          refill_map_def replaceAt_def null_def refillHd_def hd_wrap_slice
+                                          valid_refills_number'_def max_num_refills_eq_refillAbsoluteMax')
+                   apply (clarsimp simp: objBits_simps scBits_simps)
+                  apply simp
+                 apply (clarsimp simp: obj_at_simps scBits_simps is_sc_obj)
+                 apply (fastforce elim!: sc_replies_relation_prevs_list[OF state_relation_sc_replies_relation])
+                apply wpsimp
+               apply (wpsimp wp: getSchedContext_wp')
+              apply (clarsimp simp: obj_at_def is_sc_obj)
+             apply (drule state_relation_sc_relation[where ptr=sc_ptr and n=n];
+                   (fastforce simp: obj_at_simps is_sc_obj obj_bits_def)?)
+             apply (clarsimp simp: obj_at_simps is_sc_obj valid_refills_number'_def scBits_simps
+                            dest!: scRefills_length)
+            apply ((clarsimp simp: objBits_simps)+)[4]
+        (* sc_period *)
+        apply (rule corres_split[OF updateSchedContext_corres])
+             apply (fastforce dest!: state_relation_sc_relation simp: obj_at_simps is_sc_obj sc_relation_def)
+            apply (fastforce dest!: state_relation_sc_replies_relation_sc simp: obj_at_simps is_sc_obj sc_relation_def)
+           apply (simp add: objBits_simps)
+          (* sc_budget *)
+          apply (rule corres_split[OF updateSchedContext_corres])
+               apply (fastforce dest!: state_relation_sc_relation simp: obj_at_simps is_sc_obj sc_relation_def)
+              apply (fastforce dest!: state_relation_sc_replies_relation_sc simp: obj_at_simps is_sc_obj sc_relation_def)
+             apply (simp add: objBits_simps)
+            (* the rest *)
+            apply (rule_tac P="sc_obj_at n sc_ptr and
+                              (\<lambda>s. ((\<lambda>sc. sc_refills sc\<noteq> [] \<and> 0 < sc_refill_max sc) |< scs_of s) sc_ptr)"
+                       and P'="sc_at' sc_ptr and
+                              (\<lambda>s'. ((\<lambda>ko. 1 < scRefillMax ko \<and> scRefillCount ko = 1 \<and> std_sc' ko)
+                                            |< scs_of' s') sc_ptr)"
+                   in corres_inst)
+            apply (simp add: when_def[symmetric] whenM_def ifM_def bind_assoc split del: if_split)
+            apply (rule corres_guard_imp)
+              apply (rule corres_split[OF refillReady_corres]) (* projection version *)
+                (* when-block *)
+                apply (rule corres_split[OF corres_when], simp)
+                   apply (rule corres_split[OF getCurTime_corres])
+                     apply (rule corres_guard_imp)
+                       apply (rule updateRefillHd_corres, simp)
+                       apply (simp add: refill_map_def)
+                      apply (simp+)[2]
+                    apply (wpsimp+)[2]
+                  apply (simp add: liftM_def bind_assoc)
+                  apply (rule corres_split[OF get_sc_corres])
+                    (* if-block *)
+                    apply (rename_tac sc sc')
+                    apply (rule_tac P="ko_at (kernel_object.SchedContext sc n) sc_ptr
+                                        and K (0 < sc_refill_max sc) and K (sc_refills sc \<noteq> [])
+                                        and K (valid_sched_context_size n)"
+                                and P'="ko_at' sc' sc_ptr
+                                        and K (1 < scRefillMax sc' \<and> scRefillCount sc' = 1 \<and> std_sc' sc')"
+                           in corres_inst)
+                    apply (rule_tac F="refill_hd sc = refill_map (refillHd sc')" in corres_req)
+                     apply (fastforce dest!: refill_hd_relation)
+                    apply (rule corres_guard_imp)
+                      apply (rule corres_if)
+                        apply (clarsimp simp: refill_map_def)
+                       apply (rule corres_split[OF updateRefillHd_corres], simp)
+                          apply (clarsimp simp: refill_map_def)
+                         apply (rule maybeAddEmptyTail_corres)
+                        apply (wpsimp simp: update_refill_hd_rewrite)
+                       apply (wpsimp simp: updateRefillHd_def wp: updateSchedContext_wp)
+                      apply (rule refillAddTail_corres)
+                      apply (clarsimp simp: refill_map_def)
+                     apply (clarsimp simp: obj_at_def is_sc_obj is_active_sc2_def)
+                    apply (clarsimp simp: obj_at_simps  
+                                          is_sc_obj ps_clear_upd
+                                          scBits_simps fun_upd_def[symmetric])
+                   apply (clarsimp simp: obj_at'_def projectKOs objBits_simps)
+                   apply (clarsimp simp: valid_sched_context'_def valid_refills_number'_def neq_Nil_lengthI)
+                   apply wpsimp
+                  apply (wpsimp wp: getSchedContext_wp')
+                 apply (wpsimp simp: update_refill_hd_def wp: update_sched_context_wp)
+                apply (wpsimp simp: updateRefillHd_def objBits_simps
+                                wp: updateSchedContext_wp)
+               apply (wpsimp wp: get_sc_refill_ready_wp)
+              apply (wpsimp wp: refillReady_wp')
+             apply (fastforce simp: obj_at_def is_sc_obj is_active_sc2_def)
+            apply (fastforce simp: obj_at_simps ps_clear_upd fun_upd_def[symmetric])
+           apply (wpsimp wp: update_sched_context_wp)
+          apply (wpsimp wp: updateSchedContext_wp simp: objBits_simps)
+         apply (wpsimp wp: update_sched_context_wp)
+        apply (wpsimp wp: updateSchedContext_wp simp: objBits_simps)
+       apply (wpsimp wp: update_sched_context_wp)
+      apply (rule monadic_rewrite_refine_valid[where P''=\<top>, OF updateSchedContext_decompose_thrice, simplified])
+          apply ((clarsimp simp: objBits_simps)+)[4]
+      apply (wpsimp wp: updateSchedContext_wp simp: objBits_simps)
+     apply (clarsimp simp: obj_at_def is_sc_obj is_active_sc2_def)
+    apply (clarsimp simp: obj_at_simps scBits_simps ps_clear_upd fun_upd_def[symmetric]
+                          valid_refills_number'_def is_sc_obj)
+    apply (drule (1) pspace_relation_absD[OF _ state_relation_pspace_relation])
+    apply (fastforce simp: valid_sched_context'_def valid_obj'_def valid_refills_number'_def
+                           valid_sched_context_size'_def scBits_simps objBits_simps
+                    dest!: scRefills_length)
+   apply clarsimp+
   done
 
 (* FIXME RT: preconditions can be reduced, this is what is available at the call site: *)
